Restructuración por capas

examples/reordenando-la-cola-main.cs
@@ -1,0 +1,3985 @@
+// Dafny program reordenando-la-cola-main.dfy compiled into C#
+// To recompile, use 'csc' with: /r:System.Numerics.dll
+// and choosing /target:exe or /target:library
+// You might also want to include compiler switches like:
+//     /debug /nowarn:0164 /nowarn:0219 /nowarn:1717 /nowarn:0162 /nowarn:0168
+
+using System;
+using System.Numerics;
+[assembly: DafnyAssembly.DafnySourceAttribute(@"
+// Dafny 2.3.0.10506
+// Command Line Options: reordenando-la-cola-main.dfy Scan.cs
+// reordenando-la-cola-main.dfy
+
+method {:extern} Scan() returns (x: int)
+
+method ScanArray(n: nat) returns (v: array<int>)
+  ensures v.Length == n
+  ensures fresh(v)
+  decreases n
+{
+  v := new int[n];
+  var i := 0;
+  while i < n
+    decreases n - i
+  {
+    v[i] := Scan();
+    i := i + 1;
+  }
+}
+
+method {:verify false} Main()
+  decreases *
+{
+  while true
+    decreases *
+  {
+    var n := Scan();
+    if n == 0 {
+      break;
+    } else {
+      var v := ScanArray(n);
+      var neg := new Stack1();
+      var pos := new Queue1();
+      reordenandoLaCola(neg, pos, v);
+      var i := 0;
+      while i < n
+        decreases n - i
+      {
+        print v[i];
+        if i != n - 1 {
+          print "" "";
+        }
+        i := i + 1;
+      }
+      print ""\n"";
+    }
+  }
+}
+
+lemma Allocated(s: set<object>)
+  ensures forall x: object | x in s :: allocated(x)
+  decreases s
+{
+}
+
+lemma {:verify true} lemma1(v: array<int>, i: int)
+  requires forall i: int | 0 <= i < v.Length - 1 :: abs(v[i]) <= abs(v[i + 1])
+  requires 0 <= i <= v.Length
+  ensures forall j: int, k: int | 0 <= j < k < i :: abs(v[j]) <= abs(v[k])
+  decreases v, i
+{
+}
+
+method {:verify true} split(v: array<int>, neg: Stack, pos: Queue)
+  requires v !in neg.Repr() && v !in pos.Repr()
+  requires {pos} + pos.Repr() !! {neg} + neg.Repr()
+  requires neg.Valid()
+  requires pos.Valid()
+  requires neg.Empty()
+  requires pos.Empty()
+  requires forall i: int | 0 <= i < v.Length - 1 :: abs(v[i]) <= abs(v[i + 1])
+  requires forall x: object | x in neg.Repr() :: allocated(x)
+  requires forall x: object | x in pos.Repr() :: allocated(x)
+  modifies pos, pos.Repr(), neg, neg.Repr()
+  ensures v !in neg.Repr() && v !in pos.Repr()
+  ensures {pos} + pos.Repr() !! {neg} + neg.Repr()
+  ensures pos.Valid()
+  ensures neg.Valid()
+  ensures forall x: object | x in neg.Repr() - old(neg.Repr()) :: fresh(x)
+  ensures forall x: int | x in neg.Model() :: x < 0
+  ensures forall i: int | 0 <= i < |neg.Model()| - 1 :: abs(neg.Model()[i]) >= abs(neg.Model()[i + 1])
+  ensures forall x: object | x in pos.Repr() - old(pos.Repr()) :: fresh(x)
+  ensures forall x: int | x in pos.Model() :: x >= 0
+  ensures forall i: int | 0 <= i < |pos.Model()| - 1 :: abs(pos.Model()[i]) <= abs(pos.Model()[i + 1])
+  ensures Seq.MElems(neg.Model()) + Seq.MElems(pos.Model()) == Seq.MElems(v[..])
+  ensures forall x: object | x in neg.Repr() :: allocated(x)
+  ensures forall x: object | x in pos.Repr() :: allocated(x)
+  decreases v, neg, pos
+{
+  var i := 0;
+  while i < v.Length
+    invariant i <= v.Length
+    invariant forall i: int | 0 <= i < v.Length - 1 :: abs(v[i]) <= abs(v[i + 1])
+    invariant forall x: object | x in neg.Repr() - old(neg.Repr()) :: fresh(x)
+    invariant forall x: object | x in pos.Repr() - old(pos.Repr()) :: fresh(x)
+    invariant {pos} + pos.Repr() !! {neg} + neg.Repr()
+    invariant neg.Valid()
+    invariant pos.Valid()
+    invariant forall x: int | x in neg.Model() :: x < 0
+    invariant forall i: int | 0 <= i < |neg.Model()| - 1 :: abs(neg.Model()[i]) >= abs(neg.Model()[i + 1])
+    invariant forall x: int | x in pos.Model() :: x >= 0
+    invariant forall i: int | 0 <= i < |pos.Model()| - 1 :: abs(pos.Model()[i]) <= abs(pos.Model()[i + 1])
+    invariant Seq.MElems(neg.Model()) + Seq.MElems(pos.Model()) == Seq.MElems(v[..i])
+    invariant forall x: object | x in neg.Repr() :: allocated(x)
+    invariant forall x: object | x in pos.Repr() :: allocated(x)
+    decreases v.Length - i
+  {
+    lemma1(v, i + 1);
+    assert forall j: int | 0 <= j < i :: abs(v[j]) <= abs(v[i]);
+    if v[i] < 0 {
+      if |neg.Model()| > 0 {
+        assert neg.Model()[0] in Seq.MElems(neg.Model());
+        assert neg.Model()[0] in Seq.MElems(neg.Model()) + Seq.MElems(pos.Model());
+        assert neg.Model()[0] in Seq.MElems(v[..i]);
+        assert neg.Model()[0] in v[..i];
+        assert abs(v[i]) >= abs(neg.Model()[0]);
+      }
+      neg.Push(v[i]);
+    } else {
+      if |pos.Model()| > 0 {
+        assert pos.Model()[|pos.Model()| - 1] in Seq.MElems(pos.Model());
+        assert pos.Model()[|pos.Model()| - 1] in Seq.MElems(neg.Model()) + Seq.MElems(pos.Model());
+        assert pos.Model()[|pos.Model()| - 1] in Seq.MElems(v[..i]);
+        assert pos.Model()[|pos.Model()| - 1] in v[..i];
+        assert abs(pos.Model()[|pos.Model()| - 1]) <= abs(v[i]);
+      }
+      pos.Enqueue(v[i]);
+    }
+    i := i + 1;
+  }
+  assert v[..i] == v[..];
+}
+
+method {:verify true} FillFromStack(r: array<int>, i: nat, st: Stack)
+    returns (l: nat)
+  requires st.Valid()
+  requires {r} !! {st} + st.Repr()
+  requires i + |st.Model()| <= r.Length
+  requires forall x: object | x in st.Repr() :: allocated(x)
+  modifies r, st, st.Repr()
+  ensures st.Valid()
+  ensures st.Empty()
+  ensures forall x: object | x in st.Repr() - old(st.Repr()) :: fresh(x)
+  ensures forall x: object | x in st.Repr() :: allocated(x)
+  ensures r[..i] == old(r[..i])
+  ensures r[i .. i + old(|st.Model()|)] == old(st.Model())
+  ensures r[i + old(|st.Model()|)..] == old(r[i + |st.Model()|..])
+  ensures l == i + old(|st.Model()|)
+  ensures forall x: object | x in st.Repr() :: allocated(x)
+  decreases r, i, st
+{
+  l := 0;
+  while !st.Empty()
+    invariant st.Valid()
+    invariant {r} !! {st} + st.Repr()
+    invariant forall x: object | x in st.Repr() - old(st.Repr()) :: fresh(x)
+    invariant forall x: object | x in st.Repr() :: allocated(x)
+    invariant 0 <= l <= old(|st.Model()|)
+    invariant l == old(|st.Model()|) - |st.Model()|
+    invariant st.Model() == old(st.Model()[l..])
+    invariant r[..i] == old(r[..i])
+    invariant r[i .. i + l] == old(st.Model()[..l])
+    invariant r[i + old(|st.Model()|)..] == old(r[i + |st.Model()|..])
+    decreases |st.Model()|
+  {
+    var x := st.Pop();
+    r[i + l] := x;
+    l := l + 1;
+  }
+  l := l + i;
+}
+
+method {:verify true} FillFromQueue(r: array<int>, i: nat, q: Queue)
+    returns (l: nat)
+  requires q.Valid()
+  requires {r} !! {q} + q.Repr()
+  requires i + |q.Model()| <= r.Length
+  requires forall x: object | x in q.Repr() :: allocated(x)
+  modifies r, q, q.Repr()
+  ensures q.Valid()
+  ensures q.Empty()
+  ensures forall x: object | x in q.Repr() - old(q.Repr()) :: fresh(x)
+  ensures forall x: object | x in q.Repr() :: allocated(x)
+  ensures r[..i] == old(r[..i])
+  ensures r[i .. i + old(|q.Model()|)] == old(q.Model())
+  ensures r[i + old(|q.Model()|)..] == old(r[i + |q.Model()|..])
+  ensures l == i + old(|q.Model()|)
+  ensures forall x: object | x in q.Repr() :: allocated(x)
+  decreases r, i, q
+{
+  l := 0;
+  while !q.Empty()
+    invariant q.Valid()
+    invariant {r} !! {q} + q.Repr()
+    invariant forall x: object | x in q.Repr() - old(q.Repr()) :: fresh(x)
+    invariant forall x: object | x in q.Repr() :: allocated(x)
+    invariant 0 <= l <= old(|q.Model()|)
+    invariant l == old(|q.Model()|) - |q.Model()|
+    invariant q.Model() == old(q.Model()[l..])
+    invariant r[..i] == old(r[..i])
+    invariant r[i .. i + l] == old(q.Model()[..l])
+    invariant r[i + old(|q.Model()|)..] == old(r[i + |q.Model()|..])
+    decreases |q.Model()|
+  {
+    var x := q.Dequeue();
+    r[i + l] := x;
+    l := l + 1;
+  }
+  l := l + i;
+}
+
+lemma {:verify true} LastLemma(neg: seq<int>, pos: seq<int>, s: seq<int>)
+  requires forall x: int | x in neg :: x < 0
+  requires forall i: int | 0 <= i < |neg| - 1 :: abs(neg[i]) >= abs(neg[i + 1])
+  requires forall x: int | x in pos :: x >= 0
+  requires forall i: int | 0 <= i < |pos| - 1 :: abs(pos[i]) <= abs(pos[i + 1])
+  requires s == neg + pos
+  ensures forall i: int | 0 <= i < |s| - 1 :: s[i] <= s[i + 1]
+  decreases neg, pos, s
+{
+}
+
+method {:verify true} reordenandoLaCola(neg: Stack, pos: Queue, v: array<int>)
+  requires {v} !! {neg} + neg.Repr()
+  requires {v} !! {pos} + pos.Repr()
+  requires {pos} + pos.Repr() !! {neg} + neg.Repr()
+  requires forall i: int | 0 <= i < v.Length - 1 :: abs(v[i]) <= abs(v[i + 1])
+  requires neg.Valid() && neg.Empty()
+  requires pos.Valid() && pos.Empty()
+  requires forall x: object | x in neg.Repr() :: allocated(x)
+  requires forall x: object | x in pos.Repr() :: allocated(x)
+  modifies v, neg, neg.Repr(), pos, pos.Repr()
+  ensures neg.Valid()
+  ensures pos.Valid()
+  ensures {v} !! {neg} + neg.Repr()
+  ensures {v} !! {pos} + pos.Repr()
+  ensures {pos} + pos.Repr() !! {neg} + neg.Repr()
+  ensures forall x: object | x in neg.Repr() - old(neg.Repr()) :: fresh(x)
+  ensures forall x: object | x in neg.Repr() :: allocated(x)
+  ensures forall x: object | x in pos.Repr() - old(pos.Repr()) :: fresh(x)
+  ensures forall x: object | x in pos.Repr() :: allocated(x)
+  ensures Array.melems(v) == old(Array.melems(v))
+  ensures forall i: int | 0 <= i < v.Length - 1 :: v[i] <= v[i + 1]
+  decreases neg, pos, v
+{
+  split(v, neg, pos);
+  ghost var negmodel := neg.Model();
+  ghost var posmodel := pos.Model();
+  calc == {
+    |negmodel| + |posmodel|;
+    |Seq.MElems(negmodel)| + |Seq.MElems(posmodel)|;
+    |Seq.MElems(negmodel) + Seq.MElems(posmodel)|;
+    |Seq.MElems(v[..])|;
+    |v[..]|;
+    v.Length;
+  }
+  var i := 0;
+  i := FillFromStack(v, i, neg);
+  i := FillFromQueue(v, i, pos);
+  LastLemma(negmodel, posmodel, v[..]);
+}
+
+method EvalPostfix(s: string) returns (res: int)
+  requires forall c: char | c in s :: c in ""0123456789+-*//*""
+  decreases s
+{
+  var st: Stack := new Stack1();
+  var i := 0;
+  while i < |s|
+    invariant forall x: object | x in st.Repr() :: fresh(x)
+    invariant st.Valid()
+    decreases |s| - i
+  {
+    var c := s[0];
+    if c in ""0123456789"" {
+      st.Push(c as int - 48);
+    } else {
+      if st.Empty() {
+        return -1;
+      }
+      var x := st.Pop();
+      if st.Empty() {
+        return -1;
+      }
+      var y := st.Pop();
+      var n: int;
+      if c == '+' {
+        n := x + y;
+      } else if c == '-' {
+        n := x - y;
+      } else if c == '*' {
+        n := x * y;
+      } else if c == '/' {
+        if y == 0 {
+          return -1;
+        }
+        assert y != 0;
+        n := x / y;
+      }
+      st.Push(n);
+    }
+    i := i + 1;
+  }
+  if st.Empty() {
+    return -1;
+  }
+  assert !st.Empty();
+  res := st.Top();
+}
+
+function method OpeningBrace(c: char): (d: char)
+  requires c == ')' || c == ']' || c == '}'
+  decreases c
+{
+  if c == ')' then
+    '('
+  else if c == ']' then
+    '['
+  else
+    '{'
+}
+
+method BalancedTest(s: string) returns (b: bool)
+  decreases s
+{
+  var st: Stack := new Stack1();
+  var i := 0;
+  while i < |s|
+    invariant forall x: object | x in st.Repr() :: fresh(x)
+    invariant st.Valid()
+    decreases |s| - i
+  {
+    if s[i] == '(' || s[i] == '[' || s[i] == '{' {
+      st.Push(s[i] as int);
+    } else if s[i] == ')' || s[i] == ']' || s[i] == '}' {
+      if st.Empty() {
+        return false;
+      } else {
+        var c := st.Pop();
+        if c != OpeningBrace(s[i]) as int {
+          return false;
+        }
+      }
+    }
+    i := i + 1;
+  }
+  return st.Empty();
+}
+
+method Print(st: Stack)
+  requires st.Valid()
+  modifies st, st.Repr()
+  ensures st.Valid()
+  ensures st.Empty()
+  decreases st
+{
+  while !st.Empty()
+    invariant st.Valid()
+    invariant forall x: object | x in st.Repr() - old(st.Repr()) :: fresh(x)
+    decreases |st.Model()|
+  {
+    var x := st.Pop();
+    print x;
+    print ""\n"";
+  }
+}
+
+function method BigUnion<A>(S: set<set<A>>): set<A>
+  decreases S
+{
+  set X: set<A>, x: A {:trigger x in X} | X in S && x in X :: x
+}
+
+function method abs(x: int): int
+  decreases x
+{
+  if x < 0 then
+    -x
+  else
+    x
+}
+
+class Stack1 extends Stack {
+  var list: List<int>
+
+  function Depth(): nat
+  {
+    1
+  }
+
+  function Repr0(): set<object>
+    reads this
+    decreases {this}
+  {
+    {list}
+  }
+
+  function Repr1(): set<object>
+    reads this, Repr0()
+    decreases Repr0() + {this}
+  {
+    {list} + list.Repr()
+  }
+
+  function ReprFamily(n: nat): set<object>
+    reads this, if n == 0 then {} else ReprFamily(n - 1)
+    ensures n > 0 ==> ReprFamily(n) >= ReprFamily(n - 1)
+    decreases n
+  {
+    if n == 0 then
+      Repr0()
+    else if n == 1 then
+      Repr1()
+    else
+      ReprFamily(n - 1)
+  }
+
+  lemma UselessLemma()
+    ensures Repr() == ReprFamily(1)
+  {
+  }
+
+  predicate Valid()
+    reads this, Repr()
+    decreases Repr() + {this}
+  {
+    list.Valid()
+  }
+
+  function Model(): seq<int>
+    requires Valid()
+    reads this, list, list.spine
+    decreases (set _s2s_0: SNode<int> | _s2s_0 in list.spine :: _s2s_0) + {this, list}
+  {
+    list.Model()
+  }
+
+  constructor ()
+    ensures Valid()
+    ensures Model() == []
+    ensures forall x: object | x in Repr() :: fresh(x)
+    ensures forall x: object | x in Repr() :: allocated(x)
+  {
+    list := new List<int>();
+  }
+
+  function method Empty(): bool
+    requires Valid()
+    reads this, Repr()
+    ensures Empty() <==> Model() == []
+    decreases Repr() + {this}
+  {
+    list.head == null
+  }
+
+  method Top() returns (x: int)
+    requires Valid()
+    requires Model() != []
+    ensures x == Model()[0]
+  {
+    x := list.head.data;
+  }
+
+  method Push(x: int)
+    requires Valid()
+    modifies list
+    ensures Valid()
+    ensures Model() == [x] + old(Model())
+    ensures Repr() > old(Repr())
+    ensures fresh(Repr() - old(Repr()))
+    ensures list == old(list)
+    decreases x
+  {
+    list.Push(x);
+  }
+
+  method Pop() returns (x: int)
+    requires list.head != null
+    requires Valid()
+    modifies list
+    ensures Valid()
+    ensures [x] + Model() == old(Model())
+    ensures Repr() < old(Repr())
+  {
+    x := list.Pop();
+  }
+}
+
+class Queue1 extends Queue {
+  var list: DoublyLinkedListWithLast
+
+  function Depth(): nat
+    ensures Depth() > 0
+  {
+    2
+  }
+
+  function Repr0(): set<object>
+    reads this
+    decreases {this}
+  {
+    {list}
+  }
+
+  function Repr1(): set<object>
+    reads this, Repr0()
+    decreases Repr0() + {this}
+  {
+    Repr0() + {list.list}
+  }
+
+  function Repr2(): set<object>
+    reads this, Repr1()
+    decreases Repr1() + {this}
+  {
+    Repr1() + list.Repr()
+  }
+
+  function ReprFamily(n: nat): set<object>
+    requires n <= Depth()
+    reads this, if n == 0 then {} else ReprFamily(n - 1)
+    ensures n > 0 ==> ReprFamily(n) >= ReprFamily(n - 1)
+    decreases n
+  {
+    if n == 0 then
+      Repr0()
+    else if n == 1 then
+      Repr1()
+    else if n == 2 then
+      Repr2()
+    else
+      assert false; {}
+  }
+
+  predicate Valid()
+    reads this, Repr()
+    decreases Repr() + {this}
+  {
+    list.Valid()
+  }
+
+  function Model(): seq<int>
+    requires Valid()
+    reads this, Repr()
+    decreases Repr() + {this}
+  {
+    list.Model()
+  }
+
+  function method Empty(): bool
+    requires Valid()
+    reads this, Repr()
+    ensures Empty() <==> Model() == []
+    decreases Repr() + {this}
+  {
+    list.list.head == null
+  }
+
+  constructor ()
+    ensures Valid()
+    ensures Model() == []
+    ensures forall x: object | x in Repr() :: fresh(x)
+    ensures forall x: object | x in Repr() :: allocated(x)
+  {
+    list := new DoublyLinkedListWithLast();
+  }
+
+  method Front() returns (x: int)
+    requires Valid()
+    requires Model() != []
+    ensures Valid()
+    ensures Model() == old(Model())
+    ensures x == Model()[0]
+  {
+    x := list.Front();
+  }
+
+  method Enqueue(x: int)
+    requires Valid()
+    modifies Repr()
+    ensures Valid()
+    ensures Model() == old(Model()) + [x]
+    ensures Repr() > old(Repr())
+    ensures fresh(Repr() - old(Repr()))
+    decreases x
+  {
+    list.PushBack(x);
+  }
+
+  method Dequeue() returns (x: int)
+    requires Valid()
+    requires Model() != []
+    modifies Repr()
+    ensures Valid()
+    ensures [x] + Model() == old(Model())
+    ensures Repr() < old(Repr())
+  {
+    x := list.PopFront();
+  }
+}
+
+class QueueIterator {
+  ghost var index: nat
+  ghost var parent: Queue1
+  var node: DNode?
+
+  predicate Valid()
+    reads this, parent, parent.Repr()
+    decreases parent.Repr() + {this, parent}
+  {
+    parent.Valid() &&
+    (node != null ==>
+      node in parent.list.list.Repr() &&
+      index == parent.list.list.GetIndex(node))
+  }
+
+  constructor (l: Queue1)
+    requires l.Valid()
+    ensures Valid()
+    ensures parent == l
+    decreases l
+  {
+    index := 0;
+    parent := l;
+    node := l.list.list.head;
+  }
+
+  function method HasNext(): bool
+    reads this
+    decreases {this}
+  {
+    node != null
+  }
+
+  method Next() returns (x: int)
+    requires HasNext()
+    requires Valid()
+    modifies this
+    ensures Valid()
+    ensures x == old(parent.Model()[index])
+    ensures old(index) < index
+    ensures parent == old(parent)
+  {
+    {
+      parent.list.list.ModelRelationWithSpine();
+      if index < |parent.list.list.spine| - 1 {
+        assert parent.list.list.spine[index + 1] == parent.list.list.spine[index].next;
+      }
+    }
+    x := node.data;
+    index := index + 1;
+    node := node.next;
+  }
+}
+
+module Array {
+  function method elems<A>(l: array<A>): set<A>
+    reads l
+    decreases {l}, l
+  {
+    set x: A {:trigger x in l[..]} | x in l[..]
+  }
+
+  function method melems<A>(l: array<A>): multiset<A>
+    reads l
+    decreases {l}, l
+  {
+    multiset(l[..])
+  }
+}
+
+module Seq {
+  function Rev<A>(xs: seq<A>): seq<A>
+    ensures |xs| == |Rev(xs)|
+    decreases xs
+  {
+    if |xs| == 0 then
+      []
+    else
+      Rev(xs[1..]) + [xs[0]]
+  }
+
+  lemma /*{:_induction xs}*/ LeRev(xs: seq<int>)
+    requires forall i: int | 0 <= i < |xs| - 1 :: xs[i] >= xs[i + 1]
+    ensures forall i: int | 0 <= i < |xs| - 1 :: Rev(xs)[i] <= Rev(xs)[i + 1]
+    decreases xs
+  {
+  }
+
+  function Map<A, B>(f: A -> B, xs: seq<A>): seq<B>
+    reads set x: A, o: object {:trigger o in f.reads(x)} | x in xs && o in f.reads(x) :: o
+    decreases set x: A, o: object {:trigger o in f.reads(x)} | x in xs && o in f.reads(x) :: o, xs
+  {
+    if xs == [] then
+      []
+    else
+      [f(xs[0])] + Map(f, xs[1..])
+  }
+
+  function Elems<A>(xs: seq<A>): set<A>
+    decreases xs
+  {
+    set x: A {:trigger x in xs} | x in xs
+  }
+
+  lemma /*{:_induction l}*/ ElemsRev<A>(l: seq<A>)
+    ensures Elems(Rev(l)) == Elems(l)
+    ensures forall x: A | x in Rev(l) :: x in l
+    ensures forall x: A | x in l :: x in Rev(l)
+    decreases l
+  {
+  }
+
+  lemma /*{:_induction l}*/ MElemsRev<A>(l: seq<A>)
+    ensures MElems(Rev(l)) == MElems(l)
+    decreases l
+  {
+  }
+
+  function MElems<A>(xs: seq<A>): multiset<A>
+    decreases xs
+  {
+    multiset(xs)
+  }
+
+  lemma InEquivInMultiset<A>(xs: seq<A>)
+    ensures forall x: A :: x in xs <==> x in multiset(xs)
+    decreases xs
+  {
+  }
+
+  function Insert<A>(x: A, xs: seq<A>, i: nat): seq<A>
+    requires 0 <= i <= |xs|
+    ensures i == 0 ==> Insert(x, xs, i) == [x] + xs
+    ensures i == |xs| ==> Insert(x, xs, i) == xs + [x]
+    decreases xs, i
+  {
+    xs[..i] + [x] + xs[i..]
+  }
+
+  function Remove<A>(xs: seq<A>, i: nat): seq<A>
+    requires 0 <= i < |xs|
+    ensures i == 0 ==> Remove(xs, i) == xs[1..]
+    ensures i == |xs| ==> Remove(xs, i) == xs[..|xs| - 1]
+    decreases xs, i
+  {
+    xs[..i] + xs[i + 1..]
+  }
+}
+
+trait Stack {
+  function Depth(): nat
+    ensures Depth() > 0
+
+  function ReprFamily(n: nat): set<object>
+    requires n <= Depth()
+    reads this, if n == 0 then {} else ReprFamily(n - 1)
+    ensures n > 0 ==> ReprFamily(n) >= ReprFamily(n - 1)
+    decreases n
+
+  function Repr(): set<object>
+    reads this, ReprFamily(Depth() - 1)
+    decreases ReprFamily(Depth() - 1) + {this}
+  {
+    ReprFamily(Depth())
+  }
+
+  lemma UselessLemma()
+    ensures Repr() == ReprFamily(Depth())
+
+  predicate Valid()
+    reads this, Repr()
+    decreases Repr() + {this}
+
+  function Model(): seq<int>
+    requires Valid()
+    reads this, Repr()
+    decreases Repr() + {this}
+
+  function method Empty(): bool
+    requires Valid()
+    reads this, Repr()
+    ensures Empty() <==> Model() == []
+    decreases Repr() + {this}
+
+  method Top() returns (x: int)
+    requires Valid()
+    requires !Empty()
+    ensures Valid()
+    ensures Model() == old(Model())
+    ensures x == Model()[0]
+
+  method Push(x: int)
+    requires Valid()
+    modifies Repr()
+    ensures Valid()
+    ensures Model() == [x] + old(Model())
+    ensures Repr() > old(Repr())
+    ensures forall x: object | x in Repr() - old(Repr()) :: fresh(x)
+    ensures forall x: object | x in Repr() :: allocated(x)
+    decreases x
+
+  method Pop() returns (x: int)
+    requires Valid()
+    requires !Empty()
+    modifies Repr()
+    ensures Valid()
+    ensures [x] + Model() == old(Model())
+    ensures forall x: object | x in Repr() - old(Repr()) :: fresh(x)
+    ensures forall x: object | x in Repr() :: allocated(x)
+}
+
+trait Queue {
+  function Depth(): nat
+    ensures Depth() > 0
+
+  function ReprFamily(n: nat): set<object>
+    requires n <= Depth()
+    reads this, if n == 0 then {} else ReprFamily(n - 1)
+    ensures n > 0 ==> ReprFamily(n) >= ReprFamily(n - 1)
+    decreases n
+
+  function Repr(): set<object>
+    reads this, ReprFamily(Depth() - 1)
+    decreases ReprFamily(Depth() - 1) + {this}
+  {
+    ReprFamily(Depth())
+  }
+
+  predicate Valid()
+    reads this, Repr()
+    decreases Repr() + {this}
+
+  function Model(): seq<int>
+    requires Valid()
+    reads this, Repr()
+    decreases Repr() + {this}
+
+  function method Empty(): bool
+    requires Valid()
+    reads this, Repr()
+    ensures Empty() <==> Model() == []
+    decreases Repr() + {this}
+
+  method Front() returns (x: int)
+    requires Valid()
+    requires Model() != []
+    ensures Valid()
+    ensures Model() == old(Model())
+    ensures x == Model()[0]
+
+  method Enqueue(x: int)
+    requires Valid()
+    modifies Repr()
+    ensures Valid()
+    ensures Model() == old(Model()) + [x]
+    ensures forall x: object | x in Repr() - old(Repr()) :: fresh(x)
+    ensures forall x: object | x in Repr() :: allocated(x)
+    decreases x
+
+  method Dequeue() returns (x: int)
+    requires Valid()
+    requires Model() != []
+    modifies Repr()
+    ensures Valid()
+    ensures [x] + Model() == old(Model())
+    ensures forall x: object | x in Repr() - old(Repr()) :: fresh(x)
+    ensures forall x: object | x in Repr() :: allocated(x)
+}
+
+class SNode<A> {
+  var data: A
+  var next: SNode?<A>
+
+  constructor (data: A, next: SNode?<A>)
+    ensures this.data == data
+    ensures this.next == next
+    decreases next
+  {
+    this.data := data;
+    this.next := next;
+  }
+
+  predicate IsPrevOf(n: SNode<A>)
+    reads this
+    decreases {this}, n
+  {
+    next == n
+  }
+}
+
+class List<A> {
+  var head: SNode?<A>
+  ghost var spine: seq<SNode<A>>
+
+  function Repr(): set<object>
+    reads this
+    decreases {this}
+  {
+    set x: object {:trigger x in spine} | x in spine
+  }
+
+  predicate Valid()
+    reads this, Repr()
+    decreases Repr() + {this}
+  {
+    (forall i: int | 0 <= i < |spine| - 1 :: 
+      spine[i].IsPrevOf(spine[i + 1])) &&
+    if head == null then spine == [] else spine != [] && spine[0] == head && spine[|spine| - 1].next == null
+  }
+
+  lemma HeadInSpine()
+    requires Valid()
+    ensures head != null ==> head in spine
+  {
+  }
+
+  lemma DistinctSpineAux(n: nat)
+    requires Valid()
+    requires 0 <= n <= |spine|
+    ensures forall i: int, j: int | n <= i < j < |spine| :: spine[i] != spine[j]
+    decreases |spine| - n
+  {
+  }
+
+  lemma DistinctSpine()
+    requires Valid()
+    ensures forall i: int, j: int | 0 <= i < j < |spine| :: spine[i] != spine[j]
+  {
+  }
+
+  lemma HeadNotInTail()
+    requires Valid()
+    requires head != null
+    ensures head !in spine[1..]
+  {
+  }
+
+  lemma NextNullImpliesLast(n: SNode<A>)
+    requires Valid()
+    requires n in spine
+    requires n.next == null
+    ensures spine[|spine| - 1] == n
+    decreases n
+  {
+  }
+
+  lemma HeadNextNullImpliesSingleton()
+    requires Valid()
+    requires head != null
+    requires head.next == null
+    ensures spine == [head]
+  {
+  }
+
+  static function ModelAux(xs: seq<SNode<A>>): seq<A>
+    reads set x: SNode<A> {:trigger x in xs} | x in xs :: x`data
+    decreases set x: SNode<A> {:trigger x in xs} | x in xs :: x, xs
+  {
+    if xs == [] then
+      []
+    else
+      assert xs[0] in xs; assert forall x: SNode<A> | x in xs[1..] :: x in xs; [xs[0].data] + ModelAux(xs[1..])
+  }
+
+  lemma /*{:_induction xs, ys}*/ ModelAuxCommutesConcat(xs: seq<SNode<A>>, ys: seq<SNode<A>>)
+    ensures ModelAux(xs + ys) == ModelAux(xs) + ModelAux(ys)
+    decreases xs, ys
+  {
+  }
+
+  static lemma /*{:_induction spine}*/ ModelRelationWithSpineAux(spine: seq<SNode<A>>, model: seq<A>)
+    requires ModelAux(spine) == model
+    ensures |spine| == |model|
+    ensures forall i: int | 0 <= i < |spine| :: spine[i].data == model[i]
+    decreases spine, model
+  {
+  }
+
+  lemma ModelRelationWithSpine()
+    requires Valid()
+    ensures |spine| == |Model()|
+    ensures forall i: int | 0 <= i < |spine| :: spine[i].data == Model()[i]
+  {
+  }
+
+  function Model(): seq<A>
+    requires Valid()
+    reads this, spine
+    decreases (set _s2s_0: SNode<A> | _s2s_0 in spine :: _s2s_0) + {this}
+  {
+    ModelAux(spine)
+  }
+
+  static function ModelUntilAux(xs: seq<SNode<A>>, last: SNode<A>): seq<A>
+    reads set x: SNode<A> {:trigger x in xs} | x in xs :: x`data
+    decreases set x: SNode<A> {:trigger x in xs} | x in xs :: x, xs, last
+  {
+    if xs == [] || xs[0] == last then
+      []
+    else
+      assert xs[0] in xs; assert forall x: SNode<A> | x in xs[1..] :: x in xs; [xs[0].data] + ModelUntilAux(xs[1..], last)
+  }
+
+  function ModelUntil(last: SNode<A>): seq<A>
+    reads this, spine
+    decreases (set _s2s_0: SNode<A> | _s2s_0 in spine :: _s2s_0) + {this}, last
+  {
+    ModelUntilAux(spine, last)
+  }
+
+  function GetIndex(n: SNode<A>): nat
+    requires Valid()
+    requires n in Repr()
+    reads this, spine
+    ensures 0 <= GetIndex(n) < |spine|
+    ensures 0 <= GetIndex(n) < |Model()|
+    ensures spine[GetIndex(n)] == n
+    ensures forall i: int | 0 <= i < |spine| && spine[i] == n :: i == GetIndex(n)
+    decreases (set _s2s_0: SNode<A> | _s2s_0 in spine :: _s2s_0) + {this}, n
+  {
+    ModelRelationWithSpine();
+    DistinctSpine();
+    var i: int :| 0 <= i < |spine| && spine[i] == n;
+    i
+  }
+
+  lemma LastHasLastIndex(last: SNode<A>)
+    requires Valid()
+    requires last.next == null
+    requires last in Repr()
+    ensures GetIndex(last) == |spine| - 1
+    decreases last
+  {
+  }
+
+  lemma PrevHasPrevIndex(prev: SNode<A>, node: SNode<A>)
+    requires Valid()
+    requires prev in Repr()
+    requires node in Repr()
+    requires prev.IsPrevOf(node)
+    ensures GetIndex(prev) == GetIndex(node) - 1
+    decreases prev, node
+  {
+  }
+
+  constructor ()
+    ensures Valid()
+    ensures Model() == []
+    ensures fresh(Repr())
+  {
+    head := null;
+    spine := [];
+  }
+
+  method PopNode() returns (h: SNode<A>)
+    requires Valid()
+    requires Model() != []
+    modifies this
+    ensures Valid()
+    ensures [h] + spine == old(spine)
+    ensures Repr() + {h} == old(Repr())
+    ensures [h.data] + Model() == old(Model())
+    ensures Repr() < old(Repr())
+  {
+    h := head;
+    {
+      if head.next == null {
+        HeadNextNullImpliesSingleton();
+      }
+      HeadNotInTail();
+    }
+    head := head.next;
+    spine := spine[1..];
+    assert old(spine[0]) !in Repr();
+    assert old(spine[0]) in old(Repr());
+    assert Repr() < old(Repr());
+  }
+
+  method Pop() returns (res: A)
+    requires Valid()
+    requires Model() != []
+    modifies this
+    ensures Valid()
+    ensures [res] + Model() == old(Model())
+    ensures Repr() < old(Repr())
+    ensures spine == old(spine[1..])
+  {
+    var tmp := PopNode();
+    res := tmp.data;
+  }
+
+  method PushNode(h: SNode<A>)
+    requires Valid()
+    requires h !in Repr()
+    modifies this, h`next
+    ensures Valid()
+    ensures spine == [h] + old(spine)
+    ensures Model() == [h.data] + old(Model())
+    ensures Repr() > old(Repr())
+    ensures Repr() == old(Repr()) + {h}
+    decreases h
+  {
+    h.next := head;
+    head := h;
+    spine := [head] + spine;
+    assert head !in old(Repr());
+  }
+
+  method Push(x: A)
+    requires Valid()
+    modifies this
+    ensures Valid()
+    ensures Model() == [x] + old(Model())
+    ensures Repr() > old(Repr())
+    ensures fresh(Repr() - old(Repr()))
+    ensures spine[1..] == old(spine)
+  {
+    var n := new SNode<A>(x, null);
+    PushNode(n);
+  }
+
+  method Append(other: List<A>)
+    requires Valid()
+    requires other.Valid()
+    requires Repr() !! other.Repr()
+    modifies this, Repr(), other
+    ensures Valid()
+    ensures Model() == old(Model() + other.Model())
+    ensures Repr() == old(Repr() + other.Repr())
+    ensures other.Valid()
+    ensures other.Model() == []
+    ensures other.Repr() == {}
+    decreases other
+  {
+    if head == null {
+      head := other.head;
+      spine := other.spine;
+    } else {
+      var last := head;
+      ghost var i := 0;
+      while last.next != null
+        invariant last != null
+        invariant 0 <= i < |spine|
+        invariant spine[i] == last
+        decreases |spine| - i
+      {
+        last := last.next;
+        i := i + 1;
+      }
+      NextNullImpliesLast(last);
+      last.next := other.head;
+      spine := spine + other.spine;
+      ModelAuxCommutesConcat(old(spine), other.spine);
+    }
+    other.head := null;
+    other.spine := [];
+  }
+
+  method PopPush(other: List<A>)
+    requires head != null
+    requires Valid()
+    requires other.Valid()
+    requires Repr() !! other.Repr()
+    modifies this, other, Repr(), other.Repr()
+    ensures Repr() !! other.Repr()
+    ensures Valid()
+    ensures other.Valid()
+    ensures old(Repr()) > Repr()
+    ensures Repr() + {old(head)} == old(Repr())
+    ensures old(other.Repr()) < other.Repr()
+    ensures other.Repr() == old(other.Repr()) + {old(head)}
+    ensures Seq.Rev(old(Model())) + old(other.Model()) == Seq.Rev(Model()) + other.Model()
+    decreases other
+  {
+    var n := PopNode();
+    other.PushNode(n);
+  }
+
+  method Reverse()
+    requires Valid()
+    modifies this, Repr()
+    ensures Valid()
+    ensures Model() == Seq.Rev(old(Model()))
+    ensures Repr() == old(Repr())
+  {
+    var aux := new List<A>();
+    aux.head := head;
+    aux.spine := spine;
+    head := null;
+    spine := [];
+    while aux.head != null
+      invariant Valid()
+      invariant aux.Valid()
+      invariant Seq.Rev(old(Model())) == Seq.Rev(aux.Model()) + Model()
+      invariant Repr() !! aux.Repr()
+      invariant old(Repr()) == Repr() + aux.Repr()
+      decreases aux.Repr()
+    {
+      aux.PopPush(this);
+    }
+  }
+
+  method Insert(mid: SNode<A>, x: A)
+    requires Valid()
+    requires mid in Repr()
+    modifies this, mid
+    ensures Valid()
+    ensures spine == Seq.Insert(mid.next, old(spine), old(GetIndex(mid)) + 1)
+    ensures Model() == Seq.Insert(x, old(Model()), old(GetIndex(mid)) + 1)
+    ensures mid.next != null
+    ensures fresh(mid.next)
+    ensures mid.next in spine
+    ensures mid.next.next == old(mid.next)
+    ensures forall n: SNode<A> | n in old(spine) :: n in spine
+    decreases mid
+  {
+    {
+      DistinctSpine();
+      ModelRelationWithSpine();
+    }
+    var n := new SNode<A>(x, mid.next);
+    mid.next := n;
+    {
+      ghost var i :| 0 <= i < |spine| && spine[i] == mid;
+      spine := spine[..i + 1] + [n] + spine[i + 1..];
+      assert Valid();
+      ModelRelationWithSpine();
+    }
+  }
+
+  method RemoveNext(mid: SNode<A>)
+    requires Valid()
+    requires mid in Repr()
+    requires mid.next != null
+    modifies this, mid
+    ensures Valid()
+    ensures spine == Seq.Remove(old(spine), old(GetIndex(mid)) + 1)
+    ensures old(GetIndex(mid)) + 1 < old(|Model()|)
+    ensures Model() == Seq.Remove(old(Model()), old(GetIndex(mid) + 1))
+    ensures mid.next == old(mid.next.next)
+    ensures forall n: SNode<A> | n in old(spine) && n != old(mid.next) :: n in spine
+    decreases mid
+  {
+    {
+      DistinctSpine();
+      ModelRelationWithSpine();
+    }
+    ghost var i :| 0 <= i < |spine| && spine[i] == mid;
+    assert spine[i + 1] == mid.next;
+    assert i + 2 < |spine| ==> spine[i + 2] == mid.next.next;
+    mid.next := mid.next.next;
+    {
+      spine := spine[..i + 1] + spine[i + 2..];
+      assert GetIndex(mid) == old(GetIndex(mid));
+      ModelRelationWithSpine();
+      assert Model() == old(Seq.Remove(Model(), GetIndex(mid) + 1));
+    }
+  }
+
+  method FindPrev(mid: SNode<A>) returns (prev: SNode<A>)
+    requires Valid()
+    requires head != mid
+    requires mid in Repr()
+    ensures prev in Repr()
+    ensures prev.next == mid
+    decreases mid
+  {
+    prev := head;
+    ghost var i := 0;
+    while prev.next != mid
+      invariant 0 <= i < |spine|
+      invariant mid in spine[i + 1..]
+      invariant spine[i] == prev
+      decreases |spine| - i
+    {
+      assert spine[i + 1] == prev.next;
+      prev := prev.next;
+      i := i + 1;
+    }
+  }
+}
+
+class DoublyLinkedListWithLast {
+  var list: DoublyLinkedList
+  var last: DNode?
+
+  predicate Valid()
+    reads this, list, list.spine
+    decreases (set _s2s_0: DNode | _s2s_0 in list.spine :: _s2s_0) + {this, list}
+  {
+    list.Valid() &&
+    if last == null then list.head == null else last in list.Repr() && last.next == null
+  }
+
+  function Repr(): set<object>
+    reads this, list
+    decreases {this, list}
+  {
+    list.Repr()
+  }
+
+  function Model(): seq<A>
+    requires Valid()
+    reads this, list, list.spine
+    decreases (set _s2s_0: DNode | _s2s_0 in list.spine :: _s2s_0) + {this, list}
+  {
+    list.Model()
+  }
+
+  constructor ()
+    ensures Valid()
+    ensures Model() == []
+    ensures fresh(list)
+    ensures last == null
+    ensures fresh(Repr())
+  {
+    list := new DoublyLinkedList();
+    last := null;
+  }
+
+  method Front() returns (x: int)
+    requires Valid()
+    requires Model() != []
+    ensures Valid()
+    ensures Model() == old(Model())
+    ensures x == Model()[0]
+  {
+    x := list.head.data;
+  }
+
+  method Back() returns (x: int)
+    requires Valid()
+    requires Model() != []
+    ensures Valid()
+    ensures Model() == old(Model())
+    ensures x == Model()[|Model()| - 1]
+  {
+    list.LastHasLastIndex(last);
+    list.ModelRelationWithSpine();
+    x := last.data;
+  }
+
+  method PushFront(x: A)
+    requires Valid()
+    modifies this, list, Repr()
+    ensures Valid()
+    ensures Model() == [x] + old(Model())
+    ensures Repr() > old(Repr())
+    ensures fresh(Repr() - old(Repr()))
+    ensures list == old(list)
+    decreases x
+  {
+    var ohead := list.head;
+    {
+      if ohead != null {
+        list.LastHasLastIndex(last);
+      }
+    }
+    list.PushFront(x);
+    if ohead == null {
+      last := list.head;
+    }
+  }
+
+  method PopFront() returns (x: A)
+    requires Valid()
+    requires Model() != []
+    modifies this, list, Repr()
+    ensures Valid()
+    ensures [x] + Model() == old(Model())
+    ensures Repr() < old(Repr())
+    ensures list == old(list)
+  {
+    {
+      if list.head != null {
+        list.LastHasLastIndex(last);
+      }
+    }
+    if list.head == last {
+      last := null;
+    }
+    {
+      if list.head.next != null {
+        assert list.head == list.spine[0];
+        assert list.head.next == list.spine[1];
+        assert list.head.next in Repr();
+      }
+    }
+    x := list.PopFront();
+  }
+
+  method PushBack(x: A)
+    requires Valid()
+    modifies this, list, Repr()
+    ensures Valid()
+    ensures Model() == old(Model()) + [x]
+    ensures Repr() > old(Repr())
+    ensures fresh(Repr() - old(Repr()))
+    ensures list == old(list)
+    decreases x
+  {
+    if last == null {
+      assert Model() == [];
+      list.PushFront(x);
+      last := list.head;
+    } else {
+      {
+        list.LastHasLastIndex(last);
+        list.ModelRelationWithSpine();
+      }
+      list.Insert(last, x);
+      last := last.next;
+      assert last != null;
+      assert Valid();
+    }
+  }
+
+  method PopBack() returns (x: A)
+    requires Valid()
+    requires Model() != []
+    modifies this, list, list.Repr()
+    ensures Valid()
+    ensures Model() + [x] == old(Model())
+    ensures Repr() < old(Repr())
+    ensures list == old(list)
+  {
+    if list.head == last {
+      assert list.head.next == null;
+      list.HeadNextNullImpliesSingleton();
+      assert list.spine == [list.head];
+      calc == {
+        list.Model();
+        list.ModelAux(list.spine);
+        [list.head.data];
+      }
+      x := list.head.data;
+      list.head := null;
+      list.spine := [];
+      last := null;
+      assert old(list.Model()) == [x];
+      assert Model() + [x] == old(Model());
+      assert Repr() < old(Repr());
+    } else {
+      x := last.data;
+      var prev := last.prev;
+      {
+        list.ModelRelationWithSpine();
+        list.LastHasLastIndex(last);
+        assert last == list.spine[|list.spine| - 1];
+        assert last.prev == list.spine[|list.spine| - 2];
+        assert prev in Repr();
+        assert last in Repr();
+      }
+      list.RemoveNext(prev);
+      last := prev;
+    }
+  }
+}
+
+type A = int
+
+class DNode {
+  var prev: DNode?
+  var data: A
+  var next: DNode?
+
+  constructor (prev: DNode?, data: A, next: DNode?)
+    ensures this.prev == prev
+    ensures this.data == data
+    ensures this.next == next
+    decreases prev, data, next
+  {
+    this.prev := prev;
+    this.data := data;
+    this.next := next;
+  }
+
+  predicate IsPrevOf(n: DNode)
+    reads this
+    decreases {this}, n
+  {
+    next == n
+  }
+
+  predicate IsNextOf(n: DNode)
+    reads this
+    decreases {this}, n
+  {
+    prev == n
+  }
+}
+
+class DoublyLinkedList {
+  var head: DNode?
+  ghost var spine: seq<DNode>
+
+  function Repr(): set<object>
+    reads this
+    decreases {this}
+  {
+    set x: object {:trigger x in spine} | x in spine
+  }
+
+  predicate Valid()
+    reads this, Repr()
+    decreases Repr() + {this}
+  {
+    (forall i: int | 0 <= i < |spine| - 1 :: 
+      spine[i].next == spine[i + 1] &&
+      spine[i + 1].prev == spine[i]) &&
+    if head == null then spine == [] else spine != [] && spine[0] == head && spine[0].prev == null && spine[|spine| - 1].next == null
+  }
+
+  lemma DistinctSpineAux(n: nat)
+    requires Valid()
+    requires 0 <= n <= |spine|
+    ensures forall i: int, j: int | n <= i < j < |spine| :: spine[i] != spine[j]
+    decreases |spine| - n
+  {
+  }
+
+  lemma DistinctSpine()
+    requires Valid()
+    ensures forall i: int, j: int | 0 <= i < j < |spine| :: spine[i] != spine[j]
+  {
+  }
+
+  static function ModelAux(xs: seq<DNode>): seq<A>
+    reads set x: DNode {:trigger x in xs} | x in xs :: x`data
+    decreases set x: DNode {:trigger x in xs} | x in xs :: x, xs
+  {
+    if xs == [] then
+      []
+    else
+      assert xs[0] in xs; assert forall x: DNode | x in xs[1..] :: x in xs; [xs[0].data] + ModelAux(xs[1..])
+  }
+
+  lemma HeadNextNullImpliesSingleton()
+    requires Valid()
+    requires head != null
+    requires head.next == null
+    ensures spine == [head]
+  {
+  }
+
+  function Model(): seq<A>
+    requires Valid()
+    reads this, spine
+    decreases (set _s2s_0: DNode | _s2s_0 in spine :: _s2s_0) + {this}
+  {
+    ModelAux(spine)
+  }
+
+  constructor ()
+    ensures Valid()
+    ensures Model() == []
+    ensures fresh(Repr())
+  {
+    head := null;
+    spine := [];
+  }
+
+  static lemma /*{:_induction spine}*/ ModelRelationWithSpineAux(spine: seq<DNode>, model: seq<A>)
+    requires ModelAux(spine) == model
+    ensures |spine| == |model|
+    ensures forall i: int | 0 <= i < |spine| :: spine[i].data == model[i]
+    decreases spine, model
+  {
+  }
+
+  lemma ModelRelationWithSpine()
+    requires Valid()
+    ensures |spine| == |Model()|
+    ensures forall i: int | 0 <= i < |spine| :: spine[i].data == Model()[i]
+  {
+  }
+
+  function GetIndex(n: DNode): nat
+    requires Valid()
+    requires n in Repr()
+    reads this, spine
+    ensures 0 <= GetIndex(n) < |spine|
+    ensures 0 <= GetIndex(n) < |Model()|
+    ensures spine[GetIndex(n)] == n
+    ensures forall i: int | 0 <= i < |spine| && spine[i] == n :: i == GetIndex(n)
+    decreases (set _s2s_0: DNode | _s2s_0 in spine :: _s2s_0) + {this}, n
+  {
+    ModelRelationWithSpine();
+    DistinctSpine();
+    var i: int :| 0 <= i < |spine| && spine[i] == n;
+    i
+  }
+
+  lemma LastHasLastIndex(last: DNode)
+    requires Valid()
+    requires last.next == null
+    requires last in Repr()
+    ensures GetIndex(last) == |spine| - 1
+    decreases last
+  {
+  }
+
+  lemma PrevHasPrevIndex(prev: DNode, node: DNode)
+    requires Valid()
+    requires prev in Repr()
+    requires node in Repr()
+    requires prev.IsPrevOf(node)
+    ensures GetIndex(prev) == GetIndex(node) - 1
+    decreases prev, node
+  {
+  }
+
+  method PopFront() returns (x: A)
+    requires Valid()
+    requires Model() != []
+    modifies this, head.next
+    ensures Valid()
+    ensures [x] + Model() == old(Model())
+    ensures Repr() < old(Repr())
+    ensures spine == old(spine[1..])
+  {
+    DistinctSpine();
+    assert head in Repr();
+    if head.next == null {
+      HeadNextNullImpliesSingleton();
+    } else {
+      assert head == spine[0];
+      assert head.IsPrevOf(spine[1]);
+      assert spine[1] == head.next;
+      assert head.next in Repr();
+    }
+    x := head.data;
+    head := head.next;
+    spine := spine[1..];
+    if head != null {
+      head.prev := null;
+    }
+  }
+
+  method PushFront(x: A)
+    requires Valid()
+    modifies this, head
+    ensures Valid()
+    ensures Model() == [x] + old(Model())
+    ensures Repr() > old(Repr())
+    ensures fresh(Repr() - old(Repr()))
+    ensures spine[1..] == old(spine)
+    decreases x
+  {
+    var n := new DNode(null, x, head);
+    if head != null {
+      head.prev := n;
+    }
+    head := n;
+    spine := [head] + spine;
+    assert head !in old(Repr());
+  }
+
+  method Insert(mid: DNode, x: A)
+    requires Valid()
+    requires mid in Repr()
+    modifies this, Repr()
+    ensures Valid()
+    ensures spine == Seq.Insert(mid.next, old(spine), old(GetIndex(mid)) + 1)
+    ensures Model() == Seq.Insert(x, old(Model()), old(GetIndex(mid)) + 1)
+    ensures mid.next != null
+    ensures fresh(mid.next)
+    ensures mid.next in spine
+    ensures mid.next.next == old(mid.next)
+    ensures forall n: DNode | n in old(spine) :: n in spine
+    decreases mid, x
+  {
+    {
+      DistinctSpine();
+      ModelRelationWithSpine();
+    }
+    var n := new DNode(mid, x, mid.next);
+    assert n.prev == mid;
+    assert n.prev == mid;
+    ghost var i :| 0 <= i < |spine| && spine[i] == mid;
+    if mid.next != null {
+      assert spine[i + 1] == mid.next;
+      assert mid.next in Repr();
+      mid.next.prev := n;
+    }
+    mid.next := n;
+    {
+      spine := spine[..i + 1] + [n] + spine[i + 1..];
+      ModelRelationWithSpine();
+    }
+  }
+
+  method RemoveNext(mid: DNode)
+    requires Valid()
+    requires mid in Repr()
+    requires mid.next != null
+    modifies this, Repr()
+    ensures Valid()
+    ensures spine == Seq.Remove(old(spine), old(GetIndex(mid)) + 1)
+    ensures old(GetIndex(mid)) + 1 < old(|Model()|)
+    ensures Model() == Seq.Remove(old(Model()), old(GetIndex(mid) + 1))
+    ensures mid.next == old(mid.next.next)
+    ensures forall n: DNode | n in old(spine) && n != old(mid.next) :: n in spine
+    decreases mid
+  {
+    {
+      DistinctSpine();
+      ModelRelationWithSpine();
+    }
+    ghost var i :| 0 <= i < |spine| && spine[i] == mid;
+    assert spine[i + 1] == mid.next;
+    assert i + 2 < |spine| ==> spine[i + 2] == mid.next.next;
+    mid.next := mid.next.next;
+    if mid.next != null {
+      mid.next.prev := mid;
+    }
+    {
+      spine := spine[..i + 1] + spine[i + 2..];
+      assert Valid();
+      ModelRelationWithSpine();
+      assert Valid();
+      assert GetIndex(mid) == old(GetIndex(mid));
+      assert Model() == old(Seq.Remove(Model(), GetIndex(mid) + 1));
+    }
+  }
+
+  method FindPrev(mid: DNode) returns (prev: DNode)
+    requires Valid()
+    requires head != mid
+    requires mid in Repr()
+    ensures prev in Repr()
+    ensures prev.next == mid
+    decreases mid
+  {
+    prev := head;
+    ghost var i := 0;
+    while prev.next != mid
+      invariant 0 <= i < |spine|
+      invariant mid in spine[i + 1..]
+      invariant spine[i] == prev
+      decreases |spine| - i
+    {
+      assert spine[i + 1] == prev.next;
+      prev := prev.next;
+      i := i + 1;
+    }
+  }
+}
+")]
+
+#if ISDAFNYRUNTIMELIB
+using System; // for Func
+using System.Numerics;
+#endif
+
+namespace DafnyAssembly {
+  [AttributeUsage(AttributeTargets.Assembly)]
+  public class DafnySourceAttribute : Attribute {
+    public readonly string dafnySourceText;
+    public DafnySourceAttribute(string txt) { dafnySourceText = txt; }
+  }
+}
+
+namespace Dafny
+{
+  using System.Collections.Generic;
+  // set this option if you want to use System.Collections.Immutable and if you know what you're doing.
+#if DAFNY_USE_SYSTEM_COLLECTIONS_IMMUTABLE
+  using System.Collections.Immutable;
+  using System.Linq;
+#endif
+
+  public class Set<T>
+  {
+#if DAFNY_USE_SYSTEM_COLLECTIONS_IMMUTABLE
+    readonly ImmutableHashSet<T> setImpl;
+    readonly bool containsNull;
+    Set(ImmutableHashSet<T> d, bool containsNull) {
+      this.setImpl = d;
+      this.containsNull = containsNull;
+    }
+    public static readonly Set<T> Empty = new Set<T>(ImmutableHashSet<T>.Empty, false);
+    public static Set<T> FromElements(params T[] values) {
+      return FromCollection(values);
+    }
+    public static Set<T> FromCollection(IEnumerable<T> values) {
+      var d = ImmutableHashSet<T>.Empty.ToBuilder();
+      var containsNull = false;
+      foreach (T t in values) {
+        if (t == null) {
+          containsNull = true;
+        } else {
+          d.Add(t);
+        }
+      }
+      return new Set<T>(d.ToImmutable(), containsNull);
+    }
+    public static Set<T> FromCollectionPlusOne(IEnumerable<T> values, T oneMoreValue) {
+      var d = ImmutableHashSet<T>.Empty.ToBuilder();
+      var containsNull = false;
+      if (oneMoreValue == null) {
+        containsNull = true;
+      } else {
+        d.Add(oneMoreValue);
+      }
+      foreach (T t in values) {
+        if (t == null) {
+          containsNull = true;
+        } else {
+          d.Add(t);
+        }
+      }
+      return new Set<T>(d.ToImmutable(), containsNull);
+    }
+    public int Count {
+      get { return this.setImpl.Count + (containsNull ? 1 : 0); }
+    }
+    public long LongCount {
+      get { return this.setImpl.Count + (containsNull ? 1 : 0); }
+    }
+    public IEnumerable<T> Elements {
+      get {
+        if (containsNull) {
+          yield return default(T);
+        }
+        foreach (var t in this.setImpl) {
+          yield return t;
+        }
+      }
+    }
+#else
+    readonly HashSet<T> setImpl;
+    Set(HashSet<T> s) {
+      this.setImpl = s;
+    }
+    public static readonly Set<T> Empty = new Set<T>(new HashSet<T>());
+    public static Set<T> FromElements(params T[] values) {
+      return FromCollection(values);
+    }
+    public static Set<T> FromCollection(IEnumerable<T> values) {
+      var s = new HashSet<T>(values);
+      return new Set<T>(s);
+    }
+    public static Set<T> FromCollectionPlusOne(IEnumerable<T> values, T oneMoreValue) {
+      var s = new HashSet<T>(values);
+      s.Add(oneMoreValue);
+      return new Set<T>(s);
+    }
+    public int Count {
+      get { return this.setImpl.Count; }
+    }
+    public long LongCount {
+      get { return this.setImpl.Count; }
+    }
+    public IEnumerable<T> Elements {
+      get {
+        return this.setImpl;
+      }
+    }
+#endif
+
+    public static Set<T> _DafnyDefaultValue() {
+      return Empty;
+    }
+
+    /// <summary>
+    /// This is an inefficient iterator for producing all subsets of "this".
+    /// </summary>
+    public IEnumerable<Set<T>> AllSubsets {
+      get {
+        // Start by putting all set elements into a list, but don't include null
+        var elmts = new List<T>();
+        elmts.AddRange(this.setImpl);
+        var n = elmts.Count;
+        var which = new bool[n];
+#if DAFNY_USE_SYSTEM_COLLECTIONS_IMMUTABLE
+        var s = ImmutableHashSet<T>.Empty.ToBuilder();
+#else
+        var s = new HashSet<T>();
+#endif
+        while (true) {
+#if DAFNY_USE_SYSTEM_COLLECTIONS_IMMUTABLE
+          // yield both the subset without null and, if null is in the original set, the subset with null included
+          var ihs = s.ToImmutable();
+          yield return new Set<T>(ihs, false);
+          if (containsNull) {
+            yield return new Set<T>(ihs, true);
+          }
+#else
+          yield return new Set<T>(new HashSet<T>(s));
+#endif
+          // "add 1" to "which", as if doing a carry chain.  For every digit changed, change the membership of the corresponding element in "s".
+          int i = 0;
+          for (; i < n && which[i]; i++) {
+            which[i] = false;
+            s.Remove(elmts[i]);
+          }
+          if (i == n) {
+            // we have cycled through all the subsets
+            break;
+          }
+          which[i] = true;
+          s.Add(elmts[i]);
+        }
+      }
+    }
+    public bool Equals(Set<T> other) {
+#if DAFNY_USE_SYSTEM_COLLECTIONS_IMMUTABLE
+      return containsNull == other.containsNull && this.setImpl.SetEquals(other.setImpl);
+#else
+      return this.setImpl.Count == other.setImpl.Count && IsSubsetOf(other);
+#endif
+    }
+    public override bool Equals(object other) {
+      return other is Set<T> && Equals((Set<T>)other);
+    }
+    public override int GetHashCode() {
+      var hashCode = 1;
+#if DAFNY_USE_SYSTEM_COLLECTIONS_IMMUTABLE
+      if (containsNull) {
+        hashCode = hashCode * (Dafny.Helpers.GetHashCode(default(T)) + 3);
+      }
+#endif
+      foreach (var t in this.setImpl) {
+        hashCode = hashCode * (Dafny.Helpers.GetHashCode(t)+3);
+      }
+      return hashCode;
+    }
+    public override string ToString() {
+      var s = "{";
+      var sep = "";
+#if DAFNY_USE_SYSTEM_COLLECTIONS_IMMUTABLE
+      if (containsNull) {
+        s += sep + Dafny.Helpers.ToString(default(T));
+        sep = ", ";
+      }
+#endif
+      foreach (var t in this.setImpl) {
+        s += sep + Dafny.Helpers.ToString(t);
+        sep = ", ";
+      }
+      return s + "}";
+    }
+    public bool IsProperSubsetOf(Set<T> other) {
+      return this.Count < other.Count && IsSubsetOf(other);
+    }
+    public bool IsSubsetOf(Set<T> other) {
+#if DAFNY_USE_SYSTEM_COLLECTIONS_IMMUTABLE
+      if (this.containsNull && !other.containsNull) {
+        return false;
+      }
+#endif
+      if (other.setImpl.Count < this.setImpl.Count)
+        return false;
+      foreach (T t in this.setImpl) {
+        if (!other.setImpl.Contains(t))
+          return false;
+      }
+      return true;
+    }
+    public bool IsSupersetOf(Set<T> other) {
+      return other.IsSubsetOf(this);
+    }
+    public bool IsProperSupersetOf(Set<T> other) {
+      return other.IsProperSubsetOf(this);
+    }
+    public bool IsDisjointFrom(Set<T> other) {
+#if DAFNY_USE_SYSTEM_COLLECTIONS_IMMUTABLE
+      if (this.containsNull && other.containsNull) {
+        return false;
+      }
+      ImmutableHashSet<T> a, b;
+#else
+      HashSet<T> a, b;
+#endif
+      if (this.setImpl.Count < other.setImpl.Count) {
+        a = this.setImpl; b = other.setImpl;
+      } else {
+        a = other.setImpl; b = this.setImpl;
+      }
+      foreach (T t in a) {
+        if (b.Contains(t))
+          return false;
+      }
+      return true;
+    }
+    public bool Contains<G>(G t) {
+#if DAFNY_USE_SYSTEM_COLLECTIONS_IMMUTABLE
+      return t == null ? containsNull : t is T && this.setImpl.Contains((T)(object)t);
+#else
+      return (t == null || t is T) && this.setImpl.Contains((T)(object)t);
+#endif
+    }
+#if DAFNY_USE_SYSTEM_COLLECTIONS_IMMUTABLE
+    public Set<T> Union(Set<T> other) {
+      return new Set<T>(this.setImpl.Union(other.setImpl), containsNull || other.containsNull);
+    }
+    public Set<T> Intersect(Set<T> other) {
+      return new Set<T>(this.setImpl.Intersect(other.setImpl), containsNull && other.containsNull);
+    }
+    public Set<T> Difference(Set<T> other) {
+        return new Set<T>(this.setImpl.Except(other.setImpl), containsNull && !other.containsNull);
+    }
+#else
+    public Set<T> Union(Set<T> other) {
+      if (this.setImpl.Count == 0)
+        return other;
+      else if (other.setImpl.Count == 0)
+        return this;
+      HashSet<T> a, b;
+      if (this.setImpl.Count < other.setImpl.Count) {
+        a = this.setImpl; b = other.setImpl;
+      } else {
+        a = other.setImpl; b = this.setImpl;
+      }
+      var r = new HashSet<T>();
+      foreach (T t in b)
+        r.Add(t);
+      foreach (T t in a)
+        r.Add(t);
+      return new Set<T>(r);
+    }
+    public Set<T> Intersect(Set<T> other) {
+      if (this.setImpl.Count == 0)
+        return this;
+      else if (other.setImpl.Count == 0)
+        return other;
+      HashSet<T> a, b;
+      if (this.setImpl.Count < other.setImpl.Count) {
+        a = this.setImpl; b = other.setImpl;
+      } else {
+        a = other.setImpl; b = this.setImpl;
+      }
+      var r = new HashSet<T>();
+      foreach (T t in a) {
+        if (b.Contains(t))
+          r.Add(t);
+      }
+      return new Set<T>(r);
+    }
+    public Set<T> Difference(Set<T> other) {
+      if (this.setImpl.Count == 0)
+        return this;
+      else if (other.setImpl.Count == 0)
+        return this;
+      var r = new HashSet<T>();
+      foreach (T t in this.setImpl) {
+        if (!other.setImpl.Contains(t))
+          r.Add(t);
+      }
+      return new Set<T>(r);
+    }
+#endif
+  }
+
+  public class MultiSet<T>
+  {
+#if DAFNY_USE_SYSTEM_COLLECTIONS_IMMUTABLE
+    readonly ImmutableDictionary<T, int> dict;
+#else
+    readonly Dictionary<T, int> dict;
+#endif
+    readonly BigInteger occurrencesOfNull;  // stupidly, a Dictionary in .NET cannot use "null" as a key
+#if DAFNY_USE_SYSTEM_COLLECTIONS_IMMUTABLE
+    MultiSet(ImmutableDictionary<T, int>.Builder d, BigInteger occurrencesOfNull) {
+      dict = d.ToImmutable();
+      this.occurrencesOfNull = occurrencesOfNull;
+    }
+    public static readonly MultiSet<T> Empty = new MultiSet<T>(ImmutableDictionary<T, int>.Empty.ToBuilder(), BigInteger.Zero);
+#else
+    MultiSet(Dictionary<T, int> d, BigInteger occurrencesOfNull) {
+      this.dict = d;
+      this.occurrencesOfNull = occurrencesOfNull;
+    }
+    public static MultiSet<T> Empty = new MultiSet<T>(new Dictionary<T, int>(0), BigInteger.Zero);
+#endif
+    public static MultiSet<T> FromElements(params T[] values) {
+#if DAFNY_USE_SYSTEM_COLLECTIONS_IMMUTABLE
+      var d = ImmutableDictionary<T, int>.Empty.ToBuilder();
+#else
+      var d = new Dictionary<T, int>(values.Length);
+#endif
+      var occurrencesOfNull = BigInteger.Zero;
+      foreach (T t in values) {
+        if (t == null) {
+          occurrencesOfNull++;
+        } else {
+          var i = 0;
+          if (!d.TryGetValue(t, out i)) {
+            i = 0;
+          }
+          d[t] = i + 1;
+        }
+      }
+      return new MultiSet<T>(d, occurrencesOfNull);
+    }
+    public static MultiSet<T> FromCollection(ICollection<T> values) {
+#if DAFNY_USE_SYSTEM_COLLECTIONS_IMMUTABLE
+      var d = ImmutableDictionary<T, int>.Empty.ToBuilder();
+#else
+      var d = new Dictionary<T, int>();
+#endif
+      var occurrencesOfNull = BigInteger.Zero;
+      foreach (T t in values) {
+        if (t == null) {
+          occurrencesOfNull++;
+        } else {
+          var i = 0;
+          if (!d.TryGetValue(t, out i)) {
+            i = 0;
+          }
+          d[t] = i + 1;
+        }
+      }
+      return new MultiSet<T>(d, occurrencesOfNull);
+    }
+    public static MultiSet<T> FromSeq(Sequence<T> values) {
+#if DAFNY_USE_SYSTEM_COLLECTIONS_IMMUTABLE
+      var d = ImmutableDictionary<T, int>.Empty.ToBuilder();
+#else
+      var d = new Dictionary<T, int>();
+#endif
+      var occurrencesOfNull = BigInteger.Zero;
+      foreach (T t in values.Elements) {
+        if (t == null) {
+          occurrencesOfNull++;
+        } else {
+          var i = 0;
+          if (!d.TryGetValue(t, out i)) {
+            i = 0;
+          }
+          d[t] = i + 1;
+        }
+      }
+      return new MultiSet<T>(d, occurrencesOfNull);
+    }
+    public static MultiSet<T> FromSet(Set<T> values) {
+#if DAFNY_USE_SYSTEM_COLLECTIONS_IMMUTABLE
+      var d = ImmutableDictionary<T, int>.Empty.ToBuilder();
+#else
+      var d = new Dictionary<T, int>();
+#endif
+      var containsNull = false;
+      foreach (T t in values.Elements) {
+        if (t == null) {
+          containsNull = true;
+        } else {
+          d[t] = 1;
+        }
+      }
+      return new MultiSet<T>(d, containsNull ? BigInteger.One : BigInteger.Zero);
+    }
+
+    public static MultiSet<T> _DafnyDefaultValue() {
+      return Empty;
+    }
+
+    public bool Equals(MultiSet<T> other) {
+      return other.IsSubsetOf(this) && this.IsSubsetOf(other);
+    }
+    public override bool Equals(object other) {
+      return other is MultiSet<T> && Equals((MultiSet<T>)other);
+    }
+    public override int GetHashCode() {
+      var hashCode = 1;
+      if (occurrencesOfNull > 0) {
+        var key = Dafny.Helpers.GetHashCode(default(T));
+        key = (key << 3) | (key >> 29) ^ occurrencesOfNull.GetHashCode();
+        hashCode = hashCode * (key + 3);
+      }
+      foreach (var kv in dict) {
+        var key = Dafny.Helpers.GetHashCode(kv.Key);
+        key = (key << 3) | (key >> 29) ^ kv.Value.GetHashCode();
+        hashCode = hashCode * (key + 3);
+      }
+      return hashCode;
+    }
+    public override string ToString() {
+      var s = "multiset{";
+      var sep = "";
+      for (var i = BigInteger.Zero; i < occurrencesOfNull; i++) {
+        s += sep + Dafny.Helpers.ToString(default(T));
+        sep = ", ";
+      }
+      foreach (var kv in dict) {
+        var t = Dafny.Helpers.ToString(kv.Key);
+        for (int i = 0; i < kv.Value; i++) {
+          s += sep + t;
+          sep = ", ";
+        }
+      }
+      return s + "}";
+    }
+    public bool IsProperSubsetOf(MultiSet<T> other) {
+      return !Equals(other) && IsSubsetOf(other);
+    }
+    public bool IsSubsetOf(MultiSet<T> other) {
+      if (other.occurrencesOfNull < this.occurrencesOfNull) {
+        return false;
+      }
+      foreach (T t in dict.Keys) {
+        if (!other.dict.ContainsKey(t) || other.dict[t] < dict[t])
+          return false;
+      }
+      return true;
+    }
+    public bool IsSupersetOf(MultiSet<T> other) {
+      return other.IsSubsetOf(this);
+    }
+    public bool IsProperSupersetOf(MultiSet<T> other) {
+      return other.IsProperSubsetOf(this);
+    }
+    public bool IsDisjointFrom(MultiSet<T> other) {
+      if (occurrencesOfNull > 0 && other.occurrencesOfNull > 0) {
+        return false;
+      }
+      foreach (T t in dict.Keys) {
+        if (other.dict.ContainsKey(t))
+          return false;
+      }
+      foreach (T t in other.dict.Keys) {
+        if (dict.ContainsKey(t))
+          return false;
+      }
+      return true;
+    }
+
+    public bool Contains<G>(G t) {
+      return t == null ? occurrencesOfNull > 0 : t is T && dict.ContainsKey((T)(object)t);
+    }
+    public BigInteger Select<G>(G t) {
+      if (t == null) {
+        return occurrencesOfNull;
+      } else if (t is T && dict.ContainsKey((T)(object)t)) {
+        return dict[(T)(object)t];
+      } else {
+        return BigInteger.Zero;
+      }
+    }
+    public MultiSet<T> Update<G>(G t, BigInteger i) {
+      if (Select(t) == i) {
+        return this;
+      } else if (t == null) {
+#if DAFNY_USE_SYSTEM_COLLECTIONS_IMMUTABLE
+        var r = dict.ToBuilder();
+#else
+        var r = dict;
+#endif
+        return new MultiSet<T>(r, i);
+      } else {
+#if DAFNY_USE_SYSTEM_COLLECTIONS_IMMUTABLE
+        var r = dict.ToBuilder();
+#else
+        var r = new Dictionary<T, int>(dict);
+#endif
+        r[(T)(object)t] = (int)i;
+        return new MultiSet<T>(r, occurrencesOfNull);
+      }
+    }
+    public MultiSet<T> Union(MultiSet<T> other) {
+      if (dict.Count + occurrencesOfNull == 0)
+        return other;
+      else if (other.dict.Count + other.occurrencesOfNull == 0)
+        return this;
+#if DAFNY_USE_SYSTEM_COLLECTIONS_IMMUTABLE
+      var r = ImmutableDictionary<T, int>.Empty.ToBuilder();
+#else
+      var r = new Dictionary<T, int>();
+#endif
+      foreach (T t in dict.Keys) {
+        var i = 0;
+        if (!r.TryGetValue(t, out i)) {
+          i = 0;
+        }
+        r[t] = i + dict[t];
+      }
+      foreach (T t in other.dict.Keys) {
+        var i = 0;
+        if (!r.TryGetValue(t, out i)) {
+          i = 0;
+        }
+        r[t] = i + other.dict[t];
+      }
+      return new MultiSet<T>(r, occurrencesOfNull + other.occurrencesOfNull);
+    }
+    public MultiSet<T> Intersect(MultiSet<T> other) {
+      if (dict.Count == 0 && occurrencesOfNull == 0)
+        return this;
+      else if (other.dict.Count == 0 && other.occurrencesOfNull == 0)
+        return other;
+#if DAFNY_USE_SYSTEM_COLLECTIONS_IMMUTABLE
+      var r = ImmutableDictionary<T, int>.Empty.ToBuilder();
+#else
+      var r = new Dictionary<T, int>();
+#endif
+      foreach (T t in dict.Keys) {
+        if (other.dict.ContainsKey(t)) {
+          r.Add(t, other.dict[t] < dict[t] ? other.dict[t] : dict[t]);
+        }
+      }
+      return new MultiSet<T>(r, other.occurrencesOfNull < occurrencesOfNull ? other.occurrencesOfNull : occurrencesOfNull);
+    }
+    public MultiSet<T> Difference(MultiSet<T> other) { // \result == this - other
+      if (dict.Count == 0 && occurrencesOfNull == 0)
+        return this;
+      else if (other.dict.Count == 0 && other.occurrencesOfNull == 0)
+        return this;
+#if DAFNY_USE_SYSTEM_COLLECTIONS_IMMUTABLE
+      var r = ImmutableDictionary<T, int>.Empty.ToBuilder();
+#else
+      var r = new Dictionary<T, int>();
+#endif
+      foreach (T t in dict.Keys) {
+        if (!other.dict.ContainsKey(t)) {
+          r.Add(t, dict[t]);
+        } else if (other.dict[t] < dict[t]) {
+          r.Add(t, dict[t] - other.dict[t]);
+        }
+      }
+      return new MultiSet<T>(r, other.occurrencesOfNull < occurrencesOfNull ? occurrencesOfNull - other.occurrencesOfNull : BigInteger.Zero);
+    }
+
+    public int Count {
+      get { return (int)ElementCount(); }
+    }
+    public long LongCount {
+      get { return (long)ElementCount(); }
+    }
+    private BigInteger ElementCount() {
+      // This is inefficient
+      var c = occurrencesOfNull;
+      foreach (var item in dict) {
+        c += item.Value;
+      }
+      return c;
+    }
+
+    public IEnumerable<T> Elements {
+      get {
+        for (var i = BigInteger.Zero; i < occurrencesOfNull; i++) {
+          yield return default(T);
+        }
+        foreach (var item in dict) {
+          for (int i = 0; i < item.Value; i++) {
+            yield return item.Key;
+          }
+        }
+      }
+    }
+
+    public IEnumerable<T> UniqueElements {
+      get {
+        if (!occurrencesOfNull.IsZero) {
+          yield return default(T);
+        }
+        foreach (var item in dict) {
+          yield return item.Key;
+        }
+      }
+    }
+  }
+
+  public class Map<U, V>
+  {
+#if DAFNY_USE_SYSTEM_COLLECTIONS_IMMUTABLE
+    readonly ImmutableDictionary<U, V> dict;
+#else
+    readonly Dictionary<U, V> dict;
+#endif
+    readonly bool hasNullValue;  // true when "null" is a key of the Map
+    readonly V nullValue;  // if "hasNullValue", the value that "null" maps to
+
+#if DAFNY_USE_SYSTEM_COLLECTIONS_IMMUTABLE
+    Map(ImmutableDictionary<U, V>.Builder d, bool hasNullValue, V nullValue) {
+      dict = d.ToImmutable();
+      this.hasNullValue = hasNullValue;
+      this.nullValue = nullValue;
+    }
+    public static readonly Map<U, V> Empty = new Map<U, V>(ImmutableDictionary<U, V>.Empty.ToBuilder(), false, default(V));
+#else
+    Map(Dictionary<U, V> d, bool hasNullValue, V nullValue) {
+      this.dict = d;
+      this.hasNullValue = hasNullValue;
+      this.nullValue = nullValue;
+    }
+    public static readonly Map<U, V> Empty = new Map<U, V>(new Dictionary<U, V>(), false, default(V));
+#endif
+
+    public static Map<U, V> FromElements(params Pair<U, V>[] values) {
+#if DAFNY_USE_SYSTEM_COLLECTIONS_IMMUTABLE
+      var d = ImmutableDictionary<U, V>.Empty.ToBuilder();
+#else
+      var d = new Dictionary<U, V>(values.Length);
+#endif
+      var hasNullValue = false;
+      var nullValue = default(V);
+      foreach (Pair<U, V> p in values) {
+        if (p.Car == null) {
+          hasNullValue = true;
+          nullValue = p.Cdr;
+        } else {
+          d[p.Car] = p.Cdr;
+        }
+      }
+      return new Map<U, V>(d, hasNullValue, nullValue);
+    }
+    public static Map<U, V> FromCollection(List<Pair<U, V>> values) {
+#if DAFNY_USE_SYSTEM_COLLECTIONS_IMMUTABLE
+      var d = ImmutableDictionary<U, V>.Empty.ToBuilder();
+#else
+      var d = new Dictionary<U, V>(values.Count);
+#endif
+      var hasNullValue = false;
+      var nullValue = default(V);
+      foreach (Pair<U, V> p in values) {
+        if (p.Car == null) {
+          hasNullValue = true;
+          nullValue = p.Cdr;
+        } else {
+          d[p.Car] = p.Cdr;
+        }
+      }
+      return new Map<U, V>(d, hasNullValue, nullValue);
+    }
+    public int Count {
+      get { return dict.Count + (hasNullValue ? 1 : 0); }
+    }
+    public long LongCount {
+      get { return dict.Count + (hasNullValue ? 1 : 0); }
+    }
+    public static Map<U, V> _DafnyDefaultValue() {
+      return Empty;
+    }
+
+    public bool Equals(Map<U, V> other) {
+      if (hasNullValue != other.hasNullValue || dict.Count != other.dict.Count) {
+        return false;
+      } else if (hasNullValue && !Dafny.Helpers.AreEqual(nullValue, other.nullValue)) {
+        return false;
+      }
+      foreach (U u in dict.Keys) {
+        V v1 = dict[u];
+        V v2;
+        if (!other.dict.TryGetValue(u, out v2)) {
+          return false; // other dictionary does not contain this element
+        }
+        if (!Dafny.Helpers.AreEqual(v1, v2)) {
+          return false;
+        }
+      }
+      return true;
+    }
+    public override bool Equals(object other) {
+      return other is Map<U, V> && Equals((Map<U, V>)other);
+    }
+    public override int GetHashCode() {
+      var hashCode = 1;
+      if (hasNullValue) {
+        var key = Dafny.Helpers.GetHashCode(default(U));
+        key = (key << 3) | (key >> 29) ^ Dafny.Helpers.GetHashCode(nullValue);
+        hashCode = hashCode * (key + 3);
+      }
+      foreach (var kv in dict) {
+        var key = Dafny.Helpers.GetHashCode(kv.Key);
+        key = (key << 3) | (key >> 29) ^ Dafny.Helpers.GetHashCode(kv.Value);
+        hashCode = hashCode * (key + 3);
+      }
+      return hashCode;
+    }
+    public override string ToString() {
+      var s = "map[";
+      var sep = "";
+      if (hasNullValue) {
+        s += sep + Dafny.Helpers.ToString(default(U)) + " := " + Dafny.Helpers.ToString(nullValue);
+        sep = ", ";
+      }
+      foreach (var kv in dict) {
+        s += sep + Dafny.Helpers.ToString(kv.Key) + " := " + Dafny.Helpers.ToString(kv.Value);
+        sep = ", ";
+      }
+      return s + "]";
+    }
+    public bool IsDisjointFrom(Map<U, V> other) {
+      if (hasNullValue && other.hasNullValue) {
+        return false;
+      }
+      foreach (U u in dict.Keys) {
+        if (other.dict.ContainsKey(u))
+          return false;
+      }
+      foreach (U u in other.dict.Keys) {
+        if (dict.ContainsKey(u))
+          return false;
+      }
+      return true;
+    }
+    public bool Contains<G>(G u) {
+      return u == null ? hasNullValue : u is U && dict.ContainsKey((U)(object)u);
+    }
+    public V Select(U index) {
+      // evidently, the following will throw some exception if "index" in not a key of the map
+      return index == null && hasNullValue ? nullValue : dict[index];
+    }
+#if DAFNY_USE_SYSTEM_COLLECTIONS_IMMUTABLE
+    public Map<U, V> Update(U index, V val) {
+      var d = dict.ToBuilder();
+      if (index == null) {
+        return new Map<U, V>(d, true, val);
+      } else {
+        d[index] = val;
+        return new Map<U, V>(d, hasNullValue, nullValue);
+      }
+    }
+#else
+    public Map<U, V> Update(U index, V val) {
+      if (index == null) {
+        return new Map<U, V>(dict, true, val);
+      } else {
+        var d = new Dictionary<U, V>(dict);
+        d[index] = val;
+        return new Map<U, V>(d, hasNullValue, nullValue);
+      }
+    }
+#endif
+    public Set<U> Keys {
+      get {
+        if (hasNullValue) {
+          return Dafny.Set<U>.FromCollectionPlusOne(dict.Keys, default(U));
+        } else {
+          return Dafny.Set<U>.FromCollection(dict.Keys);
+        }
+      }
+    }
+    public Set<V> Values {
+      get {
+        if (hasNullValue) {
+          return Dafny.Set<V>.FromCollectionPlusOne(dict.Values, nullValue);
+        } else {
+          return Dafny.Set<V>.FromCollection(dict.Values);
+        }
+      }
+    }
+    public Set<_System.Tuple2<U, V>> Items {
+      get {
+        HashSet<_System.Tuple2<U, V>> result = new HashSet<_System.Tuple2<U, V>>();
+        if (hasNullValue) {
+          result.Add(_System.Tuple2<U, V>.create(default(U), nullValue));
+        }
+        foreach (KeyValuePair<U, V> kvp in dict) {
+          result.Add(_System.Tuple2<U, V>.create(kvp.Key, kvp.Value));
+        }
+        return Dafny.Set<_System.Tuple2<U, V>>.FromCollection(result);
+      }
+    }
+  }
+
+  public class Sequence<T>
+  {
+    readonly T[] elmts;
+    public Sequence(T[] ee) {
+      elmts = ee;
+    }
+    public static Sequence<T> Empty {
+      get {
+        return new Sequence<T>(new T[0]);
+      }
+    }
+    public static Sequence<T> FromElements(params T[] values) {
+      return new Sequence<T>(values);
+    }
+    public static Sequence<char> FromString(string s) {
+      return new Sequence<char>(s.ToCharArray());
+    }
+    public static Sequence<T> _DafnyDefaultValue() {
+      return Empty;
+    }
+    public int Count {
+      get { return elmts.Length; }
+    }
+    public long LongCount {
+      get { return elmts.LongLength; }
+    }
+    public T[] Elements {
+      get {
+        return elmts;
+      }
+    }
+    public IEnumerable<T> UniqueElements {
+      get {
+        var st = Set<T>.FromElements(elmts);
+        return st.Elements;
+      }
+    }
+    public T Select(ulong index) {
+      return elmts[index];
+    }
+    public T Select(long index) {
+      return elmts[index];
+    }
+    public T Select(uint index) {
+      return elmts[index];
+    }
+    public T Select(int index) {
+      return elmts[index];
+    }
+    public T Select(BigInteger index) {
+      return elmts[(int)index];
+    }
+    public Sequence<T> Update(long index, T t) {
+      T[] a = (T[])elmts.Clone();
+      a[index] = t;
+      return new Sequence<T>(a);
+    }
+    public Sequence<T> Update(ulong index, T t) {
+      return Update((long)index, t);
+    }
+    public Sequence<T> Update(BigInteger index, T t) {
+      return Update((long)index, t);
+    }
+    public bool Equals(Sequence<T> other) {
+      int n = elmts.Length;
+      return n == other.elmts.Length && EqualUntil(other, n);
+    }
+    public override bool Equals(object other) {
+      return other is Sequence<T> && Equals((Sequence<T>)other);
+    }
+    public override int GetHashCode() {
+      if (elmts == null || elmts.Length == 0)
+        return 0;
+      var hashCode = 0;
+      for (var i = 0; i < elmts.Length; i++) {
+        hashCode = (hashCode << 3) | (hashCode >> 29) ^ Dafny.Helpers.GetHashCode(elmts[i]);
+      }
+      return hashCode;
+    }
+    public override string ToString() {
+      if (elmts is char[]) {
+        var s = "";
+        foreach (var t in elmts) {
+          s += t.ToString();
+        }
+        return s;
+      } else {
+        var s = "[";
+        var sep = "";
+        foreach (var t in elmts) {
+          s += sep + Dafny.Helpers.ToString(t);
+          sep = ", ";
+        }
+        return s + "]";
+      }
+    }
+    bool EqualUntil(Sequence<T> other, int n) {
+      for (int i = 0; i < n; i++) {
+        if (!Dafny.Helpers.AreEqual(elmts[i], other.elmts[i]))
+          return false;
+      }
+      return true;
+    }
+    public bool IsProperPrefixOf(Sequence<T> other) {
+      int n = elmts.Length;
+      return n < other.elmts.Length && EqualUntil(other, n);
+    }
+    public bool IsPrefixOf(Sequence<T> other) {
+      int n = elmts.Length;
+      return n <= other.elmts.Length && EqualUntil(other, n);
+    }
+    public Sequence<T> Concat(Sequence<T> other) {
+      if (elmts.Length == 0)
+        return other;
+      else if (other.elmts.Length == 0)
+        return this;
+      T[] a = new T[elmts.Length + other.elmts.Length];
+      System.Array.Copy(elmts, 0, a, 0, elmts.Length);
+      System.Array.Copy(other.elmts, 0, a, elmts.Length, other.elmts.Length);
+      return new Sequence<T>(a);
+    }
+    public bool Contains<G>(G g) {
+      if (g == null || g is T) {
+        var t = (T)(object)g;
+        int n = elmts.Length;
+        for (int i = 0; i < n; i++) {
+          if (Dafny.Helpers.AreEqual(t, elmts[i]))
+            return true;
+        }
+      }
+      return false;
+    }
+    public Sequence<T> Take(long m) {
+      if (elmts.LongLength == m)
+        return this;
+      T[] a = new T[m];
+      System.Array.Copy(elmts, a, m);
+      return new Sequence<T>(a);
+    }
+    public Sequence<T> Take(ulong n) {
+      return Take((long)n);
+    }
+    public Sequence<T> Take(BigInteger n) {
+      return Take((long)n);
+    }
+    public Sequence<T> Drop(long m) {
+      if (m == 0)
+        return this;
+      T[] a = new T[elmts.Length - m];
+      System.Array.Copy(elmts, m, a, 0, elmts.Length - m);
+      return new Sequence<T>(a);
+    }
+    public Sequence<T> Drop(ulong n) {
+      return Drop((long)n);
+    }
+    public Sequence<T> Drop(BigInteger n) {
+      if (n.IsZero)
+        return this;
+      return Drop((long)n);
+    }
+  }
+  public struct Pair<A, B>
+  {
+    public readonly A Car;
+    public readonly B Cdr;
+    public Pair(A a, B b) {
+      this.Car = a;
+      this.Cdr = b;
+    }
+  }
+  public partial class Helpers {
+    public static bool AreEqual<G>(G a, G b) {
+      return a == null ? b == null : a.Equals(b);
+    }
+    public static int GetHashCode<G>(G g) {
+      return g == null ? 1001 : g.GetHashCode();
+    }
+    public static string ToString<G>(G g) {
+      if (g == null) {
+        return "null";
+      } else if (g is bool) {
+        return (bool)(object)g ? "true" : "false";  // capitalize boolean literals like in Dafny
+      } else {
+        return g.ToString();
+      }
+    }
+    public static void Print<G>(G g) {
+      System.Console.Write(ToString(g));
+    }
+    public static G Default<G>() {
+      System.Type ty = typeof(G);
+      System.Reflection.MethodInfo mInfo = ty.GetMethod("_DafnyDefaultValue");
+      if (mInfo != null) {
+        G g = (G)mInfo.Invoke(null, null);
+        return g;
+      } else {
+        return default(G);
+      }
+    }
+    // Computing forall/exists quantifiers
+    public static bool Quantifier<T>(IEnumerable<T> vals, bool frall, System.Predicate<T> pred) {
+      foreach (var u in vals) {
+        if (pred(u) != frall) { return !frall; }
+      }
+      return frall;
+    }
+    // Enumerating other collections
+    public static IEnumerable<bool> AllBooleans() {
+      yield return false;
+      yield return true;
+    }
+    public static IEnumerable<char> AllChars() {
+      for (int i = 0; i < 0x10000; i++) {
+        yield return (char)i;
+      }
+    }
+    public static IEnumerable<BigInteger> AllIntegers() {
+      yield return new BigInteger(0);
+      for (var j = new BigInteger(1);; j++) {
+        yield return j;
+        yield return -j;
+      }
+    }
+    public static IEnumerable<BigInteger> IntegerRange(Nullable<BigInteger> lo, Nullable<BigInteger> hi) {
+      if (lo == null) {
+        for (var j = (BigInteger)hi; true; ) {
+          j--;
+          yield return j;
+        }
+      } else if (hi == null) {
+        for (var j = (BigInteger)lo; true; j++) {
+          yield return j;
+        }
+      } else {
+        for (var j = (BigInteger)lo; j < hi; j++) {
+          yield return j;
+        }
+      }
+    }
+    public static IEnumerable<T> SingleValue<T>(T e) {
+      yield return e;
+    }
+    // pre: b != 0
+    // post: result == a/b, as defined by Euclidean Division (http://en.wikipedia.org/wiki/Modulo_operation)
+    public static sbyte EuclideanDivision_sbyte(sbyte a, sbyte b) {
+      return (sbyte)EuclideanDivision_int(a, b);
+    }
+    public static short EuclideanDivision_short(short a, short b) {
+      return (short)EuclideanDivision_int(a, b);
+    }
+    public static int EuclideanDivision_int(int a, int b) {
+      if (0 <= a) {
+        if (0 <= b) {
+          // +a +b: a/b
+          return (int)(((uint)(a)) / ((uint)(b)));
+        } else {
+          // +a -b: -(a/(-b))
+          return -((int)(((uint)(a)) / ((uint)(unchecked(-b)))));
+        }
+      } else {
+        if (0 <= b) {
+          // -a +b: -((-a-1)/b) - 1
+          return -((int)(((uint)(-(a + 1))) / ((uint)(b)))) - 1;
+        } else {
+          // -a -b: ((-a-1)/(-b)) + 1
+          return ((int)(((uint)(-(a + 1))) / ((uint)(unchecked(-b))))) + 1;
+        }
+      }
+    }
+    public static long EuclideanDivision_long(long a, long b) {
+      if (0 <= a) {
+        if (0 <= b) {
+          // +a +b: a/b
+          return (long)(((ulong)(a)) / ((ulong)(b)));
+        } else {
+          // +a -b: -(a/(-b))
+          return -((long)(((ulong)(a)) / ((ulong)(unchecked(-b)))));
+        }
+      } else {
+        if (0 <= b) {
+          // -a +b: -((-a-1)/b) - 1
+          return -((long)(((ulong)(-(a + 1))) / ((ulong)(b)))) - 1;
+        } else {
+          // -a -b: ((-a-1)/(-b)) + 1
+          return ((long)(((ulong)(-(a + 1))) / ((ulong)(unchecked(-b))))) + 1;
+        }
+      }
+    }
+    public static BigInteger EuclideanDivision(BigInteger a, BigInteger b) {
+      if (0 <= a.Sign) {
+        if (0 <= b.Sign) {
+          // +a +b: a/b
+          return BigInteger.Divide(a, b);
+        } else {
+          // +a -b: -(a/(-b))
+          return BigInteger.Negate(BigInteger.Divide(a, BigInteger.Negate(b)));
+        }
+      } else {
+        if (0 <= b.Sign) {
+          // -a +b: -((-a-1)/b) - 1
+          return BigInteger.Negate(BigInteger.Divide(BigInteger.Negate(a) - 1, b)) - 1;
+        } else {
+          // -a -b: ((-a-1)/(-b)) + 1
+          return BigInteger.Divide(BigInteger.Negate(a) - 1, BigInteger.Negate(b)) + 1;
+        }
+      }
+    }
+    // pre: b != 0
+    // post: result == a%b, as defined by Euclidean Division (http://en.wikipedia.org/wiki/Modulo_operation)
+    public static sbyte EuclideanModulus_sbyte(sbyte a, sbyte b) {
+      return (sbyte)EuclideanModulus_int(a, b);
+    }
+    public static short EuclideanModulus_short(short a, short b) {
+      return (short)EuclideanModulus_int(a, b);
+    }
+    public static int EuclideanModulus_int(int a, int b) {
+      uint bp = (0 <= b) ? (uint)b : (uint)(unchecked(-b));
+      if (0 <= a) {
+        // +a: a % b'
+        return (int)(((uint)a) % bp);
+      } else {
+        // c = ((-a) % b')
+        // -a: b' - c if c > 0
+        // -a: 0 if c == 0
+        uint c = ((uint)(unchecked(-a))) % bp;
+        return (int)(c == 0 ? c : bp - c);
+      }
+    }
+    public static long EuclideanModulus_long(long a, long b) {
+      ulong bp = (0 <= b) ? (ulong)b : (ulong)(unchecked(-b));
+      if (0 <= a) {
+        // +a: a % b'
+        return (long)(((ulong)a) % bp);
+      } else {
+        // c = ((-a) % b')
+        // -a: b' - c if c > 0
+        // -a: 0 if c == 0
+        ulong c = ((ulong)(unchecked(-a))) % bp;
+        return (long)(c == 0 ? c : bp - c);
+      }
+    }
+    public static BigInteger EuclideanModulus(BigInteger a, BigInteger b) {
+      var bp = BigInteger.Abs(b);
+      if (0 <= a.Sign) {
+        // +a: a % b'
+        return BigInteger.Remainder(a, bp);
+      } else {
+        // c = ((-a) % b')
+        // -a: b' - c if c > 0
+        // -a: 0 if c == 0
+        var c = BigInteger.Remainder(BigInteger.Negate(a), bp);
+        return c.IsZero ? c : BigInteger.Subtract(bp, c);
+      }
+    }
+    public static Sequence<T> SeqFromArray<T>(T[] array) {
+      return new Sequence<T>((T[])array.Clone());
+    }
+    // In .NET version 4.5, it it possible to mark a method with "AggressiveInlining", which says to inline the
+    // method if possible.  Method "ExpressionSequence" would be a good candidate for it:
+    // [System.Runtime.CompilerServices.MethodImpl(System.Runtime.CompilerServices.MethodImplOptions.AggressiveInlining)]
+    public static U ExpressionSequence<T, U>(T t, U u)
+    {
+      return u;
+    }
+
+    public static U Let<T, U>(T t, Func<T,U> f) {
+      return f(t);
+    }
+
+    public static A Id<A>(A a) {
+      return a;
+    }
+  }
+
+  public class BigOrdinal {
+    public static bool IsLimit(BigInteger ord) {
+      return ord == 0;
+    }
+    public static bool IsSucc(BigInteger ord) {
+      return 0 < ord;
+    }
+    public static BigInteger Offset(BigInteger ord) {
+      return ord;
+    }
+    public static bool IsNat(BigInteger ord) {
+      return true;  // at run time, every ORDINAL is a natural number
+    }
+  }
+
+  public struct BigRational
+  {
+    public static readonly BigRational ZERO = new BigRational(0);
+
+    // We need to deal with the special case "num == 0 && den == 0", because
+    // that's what C#'s default struct constructor will produce for BigRational. :(
+    // To deal with it, we ignore "den" when "num" is 0.
+    BigInteger num, den;  // invariant 1 <= den || (num == 0 && den == 0)
+    public override string ToString() {
+      int log10;
+      if (num.IsZero || den.IsOne) {
+        return string.Format("{0}.0", num);
+      } else if (IsPowerOf10(den, out log10)) {
+        string sign;
+        string digits;
+        if (num.Sign < 0) {
+          sign = "-"; digits = (-num).ToString();
+        } else {
+          sign = ""; digits = num.ToString();
+        }
+        if (log10 < digits.Length) {
+          var n = digits.Length - log10;
+          return string.Format("{0}{1}.{2}", sign, digits.Substring(0, n), digits.Substring(n));
+        } else {
+          return string.Format("{0}0.{1}{2}", sign, new string('0', log10 - digits.Length), digits);
+        }
+      } else {
+        return string.Format("({0}.0 / {1}.0)", num, den);
+      }
+    }
+    public bool IsPowerOf10(BigInteger x, out int log10) {
+      log10 = 0;
+      if (x.IsZero) {
+        return false;
+      }
+      while (true) {  // invariant: x != 0 && x * 10^log10 == old(x)
+        if (x.IsOne) {
+          return true;
+        } else if (x % 10 == 0) {
+          log10++;
+          x /= 10;
+        } else {
+          return false;
+        }
+      }
+    }
+    public BigRational(int n) {
+      num = new BigInteger(n);
+      den = BigInteger.One;
+    }
+    public BigRational(BigInteger n, BigInteger d) {
+      // requires 1 <= d
+      num = n;
+      den = d;
+    }
+    public BigInteger ToBigInteger() {
+      if (num.IsZero || den.IsOne) {
+        return num;
+      } else if (0 < num.Sign) {
+        return num / den;
+      } else {
+        return (num - den + 1) / den;
+      }
+    }
+    /// <summary>
+    /// Returns values such that aa/dd == a and bb/dd == b.
+    /// </summary>
+    private static void Normalize(BigRational a, BigRational b, out BigInteger aa, out BigInteger bb, out BigInteger dd) {
+      if (a.num.IsZero) {
+        aa = a.num;
+        bb = b.num;
+        dd = b.den;
+      } else if (b.num.IsZero) {
+        aa = a.num;
+        dd = a.den;
+        bb = b.num;
+      } else {
+        var gcd = BigInteger.GreatestCommonDivisor(a.den, b.den);
+        var xx = a.den / gcd;
+        var yy = b.den / gcd;
+        // We now have a == a.num / (xx * gcd) and b == b.num / (yy * gcd).
+        aa = a.num * yy;
+        bb = b.num * xx;
+        dd = a.den * yy;
+      }
+    }
+    public int CompareTo(BigRational that) {
+      // simple things first
+      int asign = this.num.Sign;
+      int bsign = that.num.Sign;
+      if (asign < 0 && 0 <= bsign) {
+        return -1;
+      } else if (asign <= 0 && 0 < bsign) {
+        return -1;
+      } else if (bsign < 0 && 0 <= asign) {
+        return 1;
+      } else if (bsign <= 0 && 0 < asign) {
+        return 1;
+      }
+      BigInteger aa, bb, dd;
+      Normalize(this, that, out aa, out bb, out dd);
+      return aa.CompareTo(bb);
+    }
+    public override int GetHashCode() {
+      return num.GetHashCode() + 29 * den.GetHashCode();
+    }
+    public override bool Equals(object obj) {
+      if (obj is BigRational) {
+        return this == (BigRational)obj;
+      } else {
+        return false;
+      }
+    }
+    public static bool operator ==(BigRational a, BigRational b) {
+      return a.CompareTo(b) == 0;
+    }
+    public static bool operator !=(BigRational a, BigRational b) {
+      return a.CompareTo(b) != 0;
+    }
+    public static bool operator >(BigRational a, BigRational b) {
+      return a.CompareTo(b) > 0;
+    }
+    public static bool operator >=(BigRational a, BigRational b) {
+      return a.CompareTo(b) >= 0;
+    }
+    public static bool operator <(BigRational a, BigRational b) {
+      return a.CompareTo(b) < 0;
+    }
+    public static bool operator <=(BigRational a, BigRational b) {
+      return a.CompareTo(b) <= 0;
+    }
+    public static BigRational operator +(BigRational a, BigRational b) {
+      BigInteger aa, bb, dd;
+      Normalize(a, b, out aa, out bb, out dd);
+      return new BigRational(aa + bb, dd);
+    }
+    public static BigRational operator -(BigRational a, BigRational b) {
+      BigInteger aa, bb, dd;
+      Normalize(a, b, out aa, out bb, out dd);
+      return new BigRational(aa - bb, dd);
+    }
+    public static BigRational operator -(BigRational a) {
+      return new BigRational(-a.num, a.den);
+    }
+    public static BigRational operator *(BigRational a, BigRational b) {
+      return new BigRational(a.num * b.num, a.den * b.den);
+    }
+    public static BigRational operator /(BigRational a, BigRational b) {
+      // Compute the reciprocal of b
+      BigRational bReciprocal;
+      if (0 < b.num.Sign) {
+        bReciprocal = new BigRational(b.den, b.num);
+      } else {
+        // this is the case b.num < 0
+        bReciprocal = new BigRational(-b.den, -b.num);
+      }
+      return a * bReciprocal;
+    }
+  }
+}
+
+namespace @_System
+{
+  public class Tuple2<T0,T1> {
+    public readonly T0 _0;
+    public readonly T1 _1;
+    public Tuple2(T0 _0, T1 _1) {
+      this._0 = _0;
+      this._1 = _1;
+    }
+    public override bool Equals(object other) {
+      var oth = other as _System.@Tuple2<T0,T1>;
+      return oth != null && Dafny.Helpers.AreEqual(this._0, oth._0) && Dafny.Helpers.AreEqual(this._1, oth._1);
+    }
+    public override int GetHashCode() {
+      ulong hash = 5381;
+      hash = ((hash << 5) + hash) + 0;
+      hash = ((hash << 5) + hash) + ((ulong)Dafny.Helpers.GetHashCode(this._0));
+      hash = ((hash << 5) + hash) + ((ulong)Dafny.Helpers.GetHashCode(this._1));
+      return (int) hash;
+    }
+    public override string ToString() {
+      string s = "";
+      s += "(";
+      s += Dafny.Helpers.ToString(this._0);
+      s += ", ";
+      s += Dafny.Helpers.ToString(this._1);
+      s += ")";
+      return s;
+    }
+    static Tuple2<T0,T1> theDefault;
+    public static Tuple2<T0,T1> Default {
+      get {
+        if (theDefault == null) {
+          theDefault = new _System.@Tuple2<T0,T1>(Dafny.Helpers.Default<T0>(), Dafny.Helpers.Default<T1>());
+        }
+        return theDefault;
+      }
+    }
+    public static Tuple2<T0,T1> _DafnyDefaultValue() { return Default; }
+    public static Tuple2<T0,T1> create(T0 _0, T1 _1) {
+      return new Tuple2<T0,T1>(_0, _1);
+    }
+    public bool is____hMake3 { get { return true; } }
+    public T0 dtor__0 {
+      get {
+        return this._0;
+      }
+    }
+    public T1 dtor__1 {
+      get {
+        return this._1;
+      }
+    }
+  }
+
+} // end of namespace _System
+namespace Dafny {
+  internal class ArrayHelpers {
+    public static T[] InitNewArray1<T>(T z, BigInteger size0) {
+      int s0 = (int)size0;
+      T[] a = new T[s0];
+      for (int i0 = 0; i0 < s0; i0++)
+        a[i0] = z;
+      return a;
+    }
+  }
+} // end of namespace Dafny
+namespace _System {
+
+
+  public partial class nat {
+  }
+
+
+
+
+
+
+
+
+  public class Tuple0 {
+    public Tuple0() {
+    }
+    public override bool Equals(object other) {
+      var oth = other as _System.Tuple0;
+      return oth != null;
+    }
+    public override int GetHashCode() {
+      ulong hash = 5381;
+      hash = ((hash << 5) + hash) + 0;
+      return (int) hash;
+    }
+    public override string ToString() {
+      return "()";
+    }
+    static Tuple0 theDefault;
+    public static Tuple0 Default {
+      get {
+        if (theDefault == null) {
+          theDefault = new _System.Tuple0();
+        }
+        return theDefault;
+      }
+    }
+    public static Tuple0 _DafnyDefaultValue() { return Default; }
+    public static Tuple0 create() {
+      return new Tuple0();
+    }
+    public bool is____hMake0 { get { return true; } }
+    public static System.Collections.Generic.IEnumerable<Tuple0> AllSingletonConstructors {
+      get {
+        yield return Tuple0.create();
+      }
+    }
+  }
+} // end of namespace _System
+namespace _0_Array_Compile {
+
+  public partial class __default {
+    public static Dafny.Set<A> elems<A>(A[] l) {
+      return ((System.Func<Dafny.Set<A>>)(() => {
+        var _coll0 = new System.Collections.Generic.List<A>();
+        foreach (var _compr_0 in (Dafny.Helpers.SeqFromArray(l)).Elements) { A _122_x = (A)_compr_0;
+          if ((Dafny.Helpers.SeqFromArray(l)).Contains(_122_x)) {
+            _coll0.Add(_122_x);
+          }
+        }
+        return Dafny.Set<A>.FromCollection(_coll0);
+      }))();
+    }
+    public static Dafny.MultiSet<A> melems<A>(A[] l) {
+      return Dafny.MultiSet<A>.FromSeq(Dafny.Helpers.SeqFromArray(l));
+    }
+  }
+} // end of namespace _0_Array_Compile
+namespace _1_Seq_Compile {
+
+} // end of namespace _1_Seq_Compile
+namespace _module {
+
+  public partial class __default {
+    public static void ScanArray(BigInteger n, out BigInteger[] v)
+    {
+    TAIL_CALL_START: ;
+      v = new BigInteger[0];
+      var _nw0 = new BigInteger[(int)(n)];
+      v = _nw0;
+      BigInteger _123_i;
+      _123_i = new BigInteger(0);
+      while ((_123_i) < (n)) {
+        BigInteger _out0;
+        __default.Scan(out _out0);
+        (v)[(int)((_123_i))] = _out0;
+        _123_i = (_123_i) + (new BigInteger(1));
+      }
+    }
+    public static void Main()
+    {
+    TAIL_CALL_START: ;
+      while (true) {
+        BigInteger _124_n;
+        BigInteger _out1;
+        __default.Scan(out _out1);
+        _124_n = _out1;
+        if ((_124_n) == (new BigInteger(0))) {
+          goto after_0;
+        } else {
+          BigInteger[] _125_v;
+          BigInteger[] _out2;
+          __default.ScanArray(_124_n, out _out2);
+          _125_v = _out2;
+          Stack1 _126_neg;
+          var _nw1 = new Stack1();
+          _nw1.__ctor();
+          _126_neg = _nw1;
+          Queue1 _127_pos;
+          var _nw2 = new Queue1();
+          _nw2.__ctor();
+          _127_pos = _nw2;
+          __default.reordenandoLaCola(_126_neg, _127_pos, _125_v);
+          BigInteger _128_i;
+          _128_i = new BigInteger(0);
+          while ((_128_i) < (_124_n)) {
+            Dafny.Helpers.Print((_125_v)[(int)(_128_i)]);
+            if ((_128_i) != ((_124_n) - (new BigInteger(1)))) {
+              Dafny.Helpers.Print(Dafny.Sequence<char>.FromString(" "));
+            }
+            _128_i = (_128_i) + (new BigInteger(1));
+          }
+          Dafny.Helpers.Print(Dafny.Sequence<char>.FromString("\n"));
+        }
+      }
+    after_0: ;
+    }
+    public static void split(BigInteger[] v, Stack neg, Queue pos)
+    {
+    TAIL_CALL_START: ;
+      BigInteger _129_i;
+      _129_i = new BigInteger(0);
+      while ((_129_i) < (new BigInteger((v).Length))) {
+        { }
+        { }
+        if (((v)[(int)(_129_i)]) < (new BigInteger(0))) {
+          { }
+          (neg).Push((v)[(int)(_129_i)]);
+        } else {
+          { }
+          (pos).Enqueue((v)[(int)(_129_i)]);
+        }
+        _129_i = (_129_i) + (new BigInteger(1));
+      }
+      { }
+    }
+    public static void FillFromStack(BigInteger[] r, BigInteger i, Stack st, out BigInteger l)
+    {
+    TAIL_CALL_START: ;
+      l = BigInteger.Zero;
+      l = new BigInteger(0);
+      while (!((st).Empty())) {
+        BigInteger _130_x;
+        BigInteger _out3;
+        (st).Pop(out _out3);
+        _130_x = _out3;
+        var _index0 = (i) + (l);
+        (r)[(int)(_index0)] = _130_x;
+        l = (l) + (new BigInteger(1));
+      }
+      l = (l) + (i);
+    }
+    public static void FillFromQueue(BigInteger[] r, BigInteger i, Queue q, out BigInteger l)
+    {
+    TAIL_CALL_START: ;
+      l = BigInteger.Zero;
+      l = new BigInteger(0);
+      while (!((q).Empty())) {
+        BigInteger _131_x;
+        BigInteger _out4;
+        (q).Dequeue(out _out4);
+        _131_x = _out4;
+        var _index1 = (i) + (l);
+        (r)[(int)(_index1)] = _131_x;
+        l = (l) + (new BigInteger(1));
+      }
+      l = (l) + (i);
+    }
+    public static void reordenandoLaCola(Stack neg, Queue pos, BigInteger[] v)
+    {
+      __default.split(v, neg, pos);
+      { }
+      { }
+      { }
+      BigInteger _132_i;
+      _132_i = new BigInteger(0);
+      BigInteger _out5;
+      __default.FillFromStack(v, _132_i, neg, out _out5);
+      _132_i = _out5;
+      BigInteger _out6;
+      __default.FillFromQueue(v, _132_i, pos, out _out6);
+      _132_i = _out6;
+      { }
+    }
+    public static void EvalPostfix(Dafny.Sequence<char> s, out BigInteger res)
+    {
+    TAIL_CALL_START: ;
+      res = BigInteger.Zero;
+      Stack _133_st;
+      var _nw3 = new Stack1();
+      _nw3.__ctor();
+      _133_st = _nw3;
+      BigInteger _134_i;
+      _134_i = new BigInteger(0);
+      while ((_134_i) < (new BigInteger((s).Count))) {
+        char _135_c;
+        _135_c = (s).Select(new BigInteger(0));
+        if ((Dafny.Sequence<char>.FromString("0123456789")).Contains(_135_c)) {
+          (_133_st).Push((new BigInteger(_135_c)) - (new BigInteger(48)));
+        } else {
+          if ((_133_st).Empty()) {
+            res = (new BigInteger(0)) - (new BigInteger(1));
+            return;
+          }
+          BigInteger _136_x;
+          BigInteger _out7;
+          (_133_st).Pop(out _out7);
+          _136_x = _out7;
+          if ((_133_st).Empty()) {
+            res = (new BigInteger(0)) - (new BigInteger(1));
+            return;
+          }
+          BigInteger _137_y;
+          BigInteger _out8;
+          (_133_st).Pop(out _out8);
+          _137_y = _out8;
+          BigInteger _138_n = BigInteger.Zero;
+          if ((_135_c) == ('+')) {
+            _138_n = (_136_x) + (_137_y);
+          } else if ((_135_c) == ('-')) {
+            _138_n = (_136_x) - (_137_y);
+          } else if ((_135_c) == ('*')) {
+            _138_n = (_136_x) * (_137_y);
+          } else if ((_135_c) == ('/')) {
+            if ((_137_y) == (new BigInteger(0))) {
+              res = (new BigInteger(0)) - (new BigInteger(1));
+              return;
+            }
+            { }
+            _138_n = Dafny.Helpers.EuclideanDivision(_136_x, _137_y);
+          }
+          (_133_st).Push(_138_n);
+        }
+        _134_i = (_134_i) + (new BigInteger(1));
+      }
+      if ((_133_st).Empty()) {
+        res = (new BigInteger(0)) - (new BigInteger(1));
+        return;
+      }
+      { }
+      BigInteger _out9;
+      (_133_st).Top(out _out9);
+      res = _out9;
+    }
+    public static char OpeningBrace(char c) {
+      if ((c) == (')')) {
+        return '(';
+      } else  {
+        if ((c) == (']')) {
+          return '[';
+        } else  {
+          return '{';
+        }
+      }
+    }
+    public static void BalancedTest(Dafny.Sequence<char> s, out bool b)
+    {
+    TAIL_CALL_START: ;
+      b = false;
+      Stack _139_st;
+      var _nw4 = new Stack1();
+      _nw4.__ctor();
+      _139_st = _nw4;
+      BigInteger _140_i;
+      _140_i = new BigInteger(0);
+      while ((_140_i) < (new BigInteger((s).Count))) {
+        if (((((s).Select(_140_i)) == ('(')) || (((s).Select(_140_i)) == ('['))) || (((s).Select(_140_i)) == ('{'))) {
+          (_139_st).Push(new BigInteger((s).Select(_140_i)));
+        } else if (((((s).Select(_140_i)) == (')')) || (((s).Select(_140_i)) == (']'))) || (((s).Select(_140_i)) == ('}'))) {
+          if ((_139_st).Empty()) {
+            b = false;
+            return;
+          } else {
+            BigInteger _141_c;
+            BigInteger _out10;
+            (_139_st).Pop(out _out10);
+            _141_c = _out10;
+            if ((_141_c) != (new BigInteger(__default.OpeningBrace((s).Select(_140_i))))) {
+              b = false;
+              return;
+            }
+          }
+        }
+        _140_i = (_140_i) + (new BigInteger(1));
+      }
+      b = (_139_st).Empty();
+      return;
+    }
+    public static void Print(Stack st)
+    {
+    TAIL_CALL_START: ;
+      while (!((st).Empty())) {
+        BigInteger _142_x;
+        BigInteger _out11;
+        (st).Pop(out _out11);
+        _142_x = _out11;
+        Dafny.Helpers.Print(_142_x);
+        Dafny.Helpers.Print(Dafny.Sequence<char>.FromString("\n"));
+      }
+    }
+    public static Dafny.Set<A> BigUnion<A>(Dafny.Set<Dafny.Set<A>> S) {
+      return ((System.Func<Dafny.Set<A>>)(() => {
+        var _coll1 = new System.Collections.Generic.List<A>();
+        foreach (var _compr_1 in (S).Elements) { Dafny.Set<A> _143_X = (Dafny.Set<A>)_compr_1;
+          foreach (var _compr_2 in (_143_X).Elements) { A _144_x = (A)_compr_2;
+            if (((S).Contains(_143_X)) && ((_143_X).Contains(_144_x))) {
+              _coll1.Add(_144_x);
+            }
+          }
+        }
+        return Dafny.Set<A>.FromCollection(_coll1);
+      }))();
+    }
+    public static BigInteger abs(BigInteger x) {
+      if ((x) < (new BigInteger(0))) {
+        return (new BigInteger(0)) - (x);
+      } else  {
+        return x;
+      }
+    }
+  }
+
+  public partial class Stack1 : Stack {
+    public List<BigInteger> list = default(List<BigInteger>);
+    public void __ctor()
+    {
+      var _this = this;
+    TAIL_CALL_START: ;
+      var _nw5 = new List<BigInteger>();
+      _nw5.__ctor();
+      (_this).list = _nw5;
+    }
+    public bool Empty() {
+      return (this.list.head) == (object) ((SNode<BigInteger>)null);
+    }
+    public void Top(out BigInteger x)
+    {
+      var _this = this;
+    TAIL_CALL_START: ;
+      x = BigInteger.Zero;
+      x = _this.list.head.data;
+    }
+    public void Push(BigInteger x)
+    {
+      var _this = this;
+    TAIL_CALL_START: ;
+      (_this.list).Push(x);
+    }
+    public void Pop(out BigInteger x)
+    {
+      var _this = this;
+    TAIL_CALL_START: ;
+      x = BigInteger.Zero;
+      BigInteger _out12;
+      (_this.list).Pop(out _out12);
+      x = _out12;
+    }
+  }
+
+  public partial class Queue1 : Queue {
+    public DoublyLinkedListWithLast list = default(DoublyLinkedListWithLast);
+    public bool Empty() {
+      return (this.list.list.head) == (object) ((DNode)null);
+    }
+    public void __ctor()
+    {
+      var _this = this;
+    TAIL_CALL_START: ;
+      var _nw6 = new DoublyLinkedListWithLast();
+      _nw6.__ctor();
+      (_this).list = _nw6;
+    }
+    public void Front(out BigInteger x)
+    {
+      var _this = this;
+    TAIL_CALL_START: ;
+      x = BigInteger.Zero;
+      BigInteger _out13;
+      (_this.list).Front(out _out13);
+      x = _out13;
+    }
+    public void Enqueue(BigInteger x)
+    {
+      var _this = this;
+    TAIL_CALL_START: ;
+      (_this.list).PushBack(x);
+    }
+    public void Dequeue(out BigInteger x)
+    {
+      var _this = this;
+    TAIL_CALL_START: ;
+      x = BigInteger.Zero;
+      BigInteger _out14;
+      (_this.list).PopFront(out _out14);
+      x = _out14;
+    }
+  }
+
+  public partial class QueueIterator {
+    public DNode node = (DNode)null;
+    public void __ctor(Queue1 l)
+    {
+      var _this = this;
+    TAIL_CALL_START: ;
+      { }
+      { }
+      (_this).node = l.list.list.head;
+    }
+    public bool HasNext() {
+      return (this.node) != (object) ((DNode)null);
+    }
+    public void Next(out BigInteger x)
+    {
+      var _this = this;
+    TAIL_CALL_START: ;
+      x = BigInteger.Zero;
+      { }
+      x = _this.node.data;
+      { }
+      (_this).node = _this.node.next;
+    }
+  }
+
+
+
+  public interface Stack {
+    bool Empty();
+    void Top(out BigInteger x);
+    void Push(BigInteger x);
+    void Pop(out BigInteger x);
+  }
+  public class _Companion_Stack {
+  }
+
+  public interface Queue {
+    bool Empty();
+    void Front(out BigInteger x);
+    void Enqueue(BigInteger x);
+    void Dequeue(out BigInteger x);
+  }
+  public class _Companion_Queue {
+  }
+
+  public partial class SNode<A> {
+    public A data = Dafny.Helpers.Default<A>();
+    public SNode<A> next = (SNode<A>)null;
+    public void __ctor(A data, SNode<A> next)
+    {
+      var _this = this;
+    TAIL_CALL_START: ;
+      (_this).data = data;
+      (_this).next = next;
+    }
+  }
+
+  public partial class List<A> {
+    public SNode<A> head = (SNode<A>)null;
+    public void __ctor()
+    {
+      var _this = this;
+    TAIL_CALL_START: ;
+      (_this).head = (SNode<A>)null;
+      { }
+    }
+    public void PopNode(out SNode<A> h)
+    {
+      var _this = this;
+    TAIL_CALL_START: ;
+      h = default(SNode<A>);
+      h = _this.head;
+      { }
+      (_this).head = _this.head.next;
+      { }
+      { }
+      { }
+      { }
+    }
+    public void Pop(out A res)
+    {
+      var _this = this;
+    TAIL_CALL_START: ;
+      res = Dafny.Helpers.Default<A>();
+      SNode<A> _145_tmp;
+      SNode<A> _out15;
+      (_this).PopNode(out _out15);
+      _145_tmp = _out15;
+      res = _145_tmp.data;
+    }
+    public void PushNode(SNode<A> h)
+    {
+      var _this = this;
+    TAIL_CALL_START: ;
+      (h).next = _this.head;
+      (_this).head = h;
+      { }
+      { }
+    }
+    public void Push(A x)
+    {
+      var _this = this;
+    TAIL_CALL_START: ;
+      SNode<A> _146_n;
+      var _nw7 = new SNode<A>();
+      _nw7.__ctor(x, (SNode<A>)null);
+      _146_n = _nw7;
+      (_this).PushNode(_146_n);
+    }
+    public void Append(List<A> other)
+    {
+      if ((this.head) == (object) ((SNode<A>)null)) {
+        (this).head = other.head;
+        { }
+      } else {
+        SNode<A> _147_last;
+        _147_last = this.head;
+        { }
+        while ((_147_last.next) != (object) ((SNode<A>)null)) {
+          _147_last = _147_last.next;
+          { }
+        }
+        { }
+        (_147_last).next = other.head;
+        { }
+        { }
+      }
+      (other).head = (SNode<A>)null;
+      { }
+    }
+    public void PopPush(List<A> other)
+    {
+      var _this = this;
+    TAIL_CALL_START: ;
+      SNode<A> _148_n;
+      SNode<A> _out16;
+      (_this).PopNode(out _out16);
+      _148_n = _out16;
+      (other).PushNode(_148_n);
+    }
+    public void Reverse()
+    {
+      var _this = this;
+    TAIL_CALL_START: ;
+      List<A> _149_aux;
+      var _nw8 = new List<A>();
+      _nw8.__ctor();
+      _149_aux = _nw8;
+      (_149_aux).head = _this.head;
+      { }
+      (_this).head = (SNode<A>)null;
+      { }
+      while ((_149_aux.head) != (object) ((SNode<A>)null)) {
+        (_149_aux).PopPush(_this);
+      }
+    }
+    public void Insert(SNode<A> mid, A x)
+    {
+      { }
+      SNode<A> _150_n;
+      var _nw9 = new SNode<A>();
+      _nw9.__ctor(x, mid.next);
+      _150_n = _nw9;
+      (mid).next = _150_n;
+      {
+        { }
+        { }
+        { }
+        { }
+      }
+    }
+    public void RemoveNext(SNode<A> mid)
+    {
+      { }
+      { }
+      { }
+      { }
+      (mid).next = mid.next.next;
+      { }
+    }
+    public void FindPrev(SNode<A> mid, out SNode<A> prev)
+    {
+      prev = default(SNode<A>);
+      prev = this.head;
+      { }
+      while ((prev.next) != (object) (mid)) {
+        { }
+        prev = prev.next;
+        { }
+      }
+    }
+  }
+
+  public partial class DoublyLinkedListWithLast {
+    public DoublyLinkedList list = default(DoublyLinkedList);
+    public DNode last = (DNode)null;
+    public void __ctor()
+    {
+      var _this = this;
+    TAIL_CALL_START: ;
+      var _nw10 = new DoublyLinkedList();
+      _nw10.__ctor();
+      (_this).list = _nw10;
+      (_this).last = (DNode)null;
+    }
+    public void Front(out BigInteger x)
+    {
+      var _this = this;
+    TAIL_CALL_START: ;
+      x = BigInteger.Zero;
+      x = _this.list.head.data;
+    }
+    public void Back(out BigInteger x)
+    {
+      var _this = this;
+    TAIL_CALL_START: ;
+      x = BigInteger.Zero;
+      { }
+      { }
+      x = _this.last.data;
+    }
+    public void PushFront(BigInteger x)
+    {
+      var _this = this;
+    TAIL_CALL_START: ;
+      DNode _151_ohead;
+      _151_ohead = _this.list.head;
+      { }
+      (_this.list).PushFront(x);
+      if ((_151_ohead) == (object) ((DNode)null)) {
+        (_this).last = _this.list.head;
+      }
+    }
+    public void PopFront(out BigInteger x)
+    {
+      var _this = this;
+    TAIL_CALL_START: ;
+      x = BigInteger.Zero;
+      { }
+      if ((_this.list.head) == (object) (_this.last)) {
+        (_this).last = (DNode)null;
+      }
+      { }
+      BigInteger _out17;
+      (_this.list).PopFront(out _out17);
+      x = _out17;
+    }
+    public void PushBack(BigInteger x)
+    {
+      var _this = this;
+    TAIL_CALL_START: ;
+      if ((_this.last) == (object) ((DNode)null)) {
+        { }
+        (_this.list).PushFront(x);
+        (_this).last = _this.list.head;
+      } else {
+        { }
+        (_this.list).Insert(_this.last, x);
+        (_this).last = _this.last.next;
+        { }
+        { }
+      }
+    }
+    public void PopBack(out BigInteger x)
+    {
+      var _this = this;
+    TAIL_CALL_START: ;
+      x = BigInteger.Zero;
+      if ((_this.list.head) == (object) (_this.last)) {
+        { }
+        { }
+        { }
+        { }
+        x = _this.list.head.data;
+        var _obj0 = _this.list;
+        _obj0.head = (DNode)null;
+        { }
+        (_this).last = (DNode)null;
+        { }
+        { }
+        { }
+      } else {
+        x = _this.last.data;
+        DNode _152_prev;
+        _152_prev = _this.last.prev;
+        { }
+        (_this.list).RemoveNext(_152_prev);
+        (_this).last = _152_prev;
+      }
+    }
+  }
+
+
+  public partial class DNode {
+    public DNode prev = (DNode)null;
+    public BigInteger data = BigInteger.Zero;
+    public DNode next = (DNode)null;
+    public void __ctor(DNode prev, BigInteger data, DNode next)
+    {
+      var _this = this;
+    TAIL_CALL_START: ;
+      (_this).prev = prev;
+      (_this).data = data;
+      (_this).next = next;
+    }
+  }
+
+  public partial class DoublyLinkedList {
+    public DNode head = (DNode)null;
+    public void __ctor()
+    {
+      var _this = this;
+    TAIL_CALL_START: ;
+      (_this).head = (DNode)null;
+      { }
+    }
+    public void PopFront(out BigInteger x)
+    {
+      var _this = this;
+    TAIL_CALL_START: ;
+      x = BigInteger.Zero;
+      { }
+      { }
+      { }
+      x = _this.head.data;
+      (_this).head = _this.head.next;
+      { }
+      if ((_this.head) != (object) ((DNode)null)) {
+        var _obj1 = _this.head;
+        _obj1.prev = (DNode)null;
+      }
+    }
+    public void PushFront(BigInteger x)
+    {
+      var _this = this;
+    TAIL_CALL_START: ;
+      DNode _153_n;
+      var _nw11 = new DNode();
+      _nw11.__ctor((DNode)null, x, _this.head);
+      _153_n = _nw11;
+      if ((_this.head) != (object) ((DNode)null)) {
+        var _obj2 = _this.head;
+        _obj2.prev = _153_n;
+      }
+      (_this).head = _153_n;
+      { }
+      { }
+    }
+    public void Insert(DNode mid, BigInteger x)
+    {
+      { }
+      DNode _154_n;
+      var _nw12 = new DNode();
+      _nw12.__ctor(mid, x, mid.next);
+      _154_n = _nw12;
+      { }
+      { }
+      { }
+      if ((mid.next) != (object) ((DNode)null)) {
+        { }
+        { }
+        var _obj3 = mid.next;
+        _obj3.prev = _154_n;
+      }
+      (mid).next = _154_n;
+      { }
+    }
+    public void RemoveNext(DNode mid)
+    {
+      { }
+      { }
+      { }
+      { }
+      (mid).next = mid.next.next;
+      if ((mid.next) != (object) ((DNode)null)) {
+        var _obj4 = mid.next;
+        _obj4.prev = mid;
+      }
+      { }
+    }
+    public void FindPrev(DNode mid, out DNode prev)
+    {
+      prev = default(DNode);
+      prev = this.head;
+      { }
+      while ((prev.next) != (object) (mid)) {
+        { }
+        prev = prev.next;
+        { }
+      }
+    }
+  }
+} // end of namespace _module
