src/linear/aux/DoublyLinkedListWithLast.dfy
@@ -1,8 +1,19 @@
-include "../../../src/linear/implementation/SinglyLinkedListWithSpine.dfy"
+include "../../../src/linear/aux/DoublyLinkedList.dfy"
 
-class SinglyLinkedListWithLast<A> {
-  var list: List<A>;
-  var last: SNode?<A>;
+class DoublyLinkedListWithLast {
+  var list: DoublyLinkedList;
+  var last: DNode?;
+
+  predicate Valid()
+    reads this, list, list.spine
+  {
+    && list.Valid()
+    && (if last == null then
+        list.head == null
+      else
+        last in list.Repr() && last.next == null
+      )
+  }
 
   function Repr(): set<object>
     reads this, list
@@ -10,19 +21,8 @@ class SinglyLinkedListWithLast<A> {
     list.Repr()
   }
 
-  predicate Valid()
-    reads this, list, Repr()
-  {
-    && list.Valid()
-      && (if last == null then
-      list.head == null
-      else
-        last in list.Repr() && last.next == null
-        )
-  }
-
   function Model(): seq<A>
-    reads this, list, Repr()
+    reads this, list, list.spine
     requires Valid()
   {
     list.Model()
@@ -31,16 +31,16 @@ class SinglyLinkedListWithLast<A> {
   constructor()
     ensures Valid()
     ensures Model() == []
-    ensures fresh(Repr())
     ensures fresh(list)
     ensures last == null
+    ensures fresh(Repr())
   {
-    list := new List();
+    list := new DoublyLinkedList();
     last := null;
   }
 
-  function method Front(): A
-    reads this, list, Repr()
+  function method Front(): int
+    reads this, list, list.Repr()
     requires Valid()
     requires Model() != []
     ensures Valid()
@@ -49,9 +49,21 @@ class SinglyLinkedListWithLast<A> {
     list.head.data
   }
 
+  function method Back(): int
+    reads this, list, list.Repr()
+    requires Valid()
+    requires Model() != []
+    ensures Valid()
+    ensures Back() == Model()[|Model()|-1]
+  {
+    list.LastHasLastIndex(last);
+    list.ModelRelationWithSpine();
+    last.data
+  }
+
   // O(1)
   method PushFront(x: A)
-    modifies this, list
+    modifies this, list, Repr()
     requires Valid()
     ensures Valid()
     ensures Model() == [x] + old(Model())
@@ -60,7 +72,12 @@ class SinglyLinkedListWithLast<A> {
     ensures list == old(list)
   {
     var ohead := list.head;
-    list.Push(x);
+    { // GHOST
+      if ohead != null {
+        list.LastHasLastIndex(last);
+      }
+    }
+    list.PushFront(x);
     if ohead == null {
       last := list.head;
     }
@@ -68,23 +85,36 @@ class SinglyLinkedListWithLast<A> {
 
   // O(1)
   method PopFront() returns (x: A)
-    modifies this, list
+    modifies this, list, Repr()
     requires Valid()
     requires Model() != []
     ensures Valid()
     ensures [x] + Model() == old(Model())
     ensures Repr() < old(Repr())
     ensures list == old(list)
+    ensures [old(list.head)] + list.spine == old(list.spine);
   {
+    { // GHOST
+      if list.head != null {
+        list.LastHasLastIndex(last);
+      }
+    }
     if list.head == last {
       last := null;
     }
-    x := list.Pop();
+    { // GHOST
+      if list.head.next != null {
+        assert list.head == list.spine[0];
+        assert list.head.next == list.spine[1];
+        assert list.head.next in Repr();
+      }
+    }
+    x := list.PopFront();
   }
 
   // O(1)
   method PushBack(x: A)
-    modifies this, last, list
+    modifies this, list, Repr()
     requires Valid()
     ensures Valid()
     ensures Model() == old(Model()) + [x]
@@ -94,7 +124,7 @@ class SinglyLinkedListWithLast<A> {
   {
     if last == null {
       assert Model() == [];
-      list.Push(x);
+      list.PushFront(x);
       last := list.head;
     } else {
       { // GHOST
@@ -108,7 +138,7 @@ class SinglyLinkedListWithLast<A> {
     }
   }
 
-  // O(n)
+  // O(1)
   method PopBack() returns (x: A)
     modifies this, list, list.Repr()
     requires Valid()
@@ -117,6 +147,7 @@ class SinglyLinkedListWithLast<A> {
     ensures Model() + [x] == old(Model())
     ensures Repr() < old(Repr())
     ensures list == old(list)
+    ensures list.spine + [old(last)] == old(list.spine)
   {
     if list.head == last {
       assert list.head.next == null;
@@ -135,15 +166,18 @@ class SinglyLinkedListWithLast<A> {
       assert Model() + [x] == old(Model());
       assert Repr() < old(Repr());
     } else {
-      /*GHOST*/ list.ModelRelationWithSpine();
-      var prev := list.FindPrev(last);
-      assert prev in Repr();
-      assert last in Repr();
-      /*GHOST*/ list.PrevHasPrevIndex(prev, last);
-      list.RemoveNext(prev);
       x := last.data;
+      var prev := last.prev;
+      { // GHOST
+        list.ModelRelationWithSpine();
+        list.LastHasLastIndex(last);
+        assert last == list.spine[|list.spine|-1];
+        assert last.prev == list.spine[|list.spine|-2];
+        assert prev in Repr();
+        assert last in Repr();
+      }
+      list.RemoveNext(prev);
       last := prev;
-      /*GHOST*/ list.LastHasLastIndex(last);
     }
   }
 }
