src/linear/aux/SinglyLinkedListWithLast.dfy
@@ -1,19 +1,8 @@
-include "../../../src/linear/implementation/DoublyLinkedList.dfy"
+include "../../../src/linear/aux/SinglyLinkedListWithSpine.dfy"
 
-class DoublyLinkedListWithLast {
-  var list: DoublyLinkedList;
-  var last: DNode?;
-
-  predicate Valid()
-    reads this, list, list.spine
-  {
-    && list.Valid()
-    && (if last == null then
-        list.head == null
-      else
-        last in list.Repr() && last.next == null
-      )
-  }
+class SinglyLinkedListWithLast<A> {
+  var list: List<A>;
+  var last: SNode?<A>;
 
   function Repr(): set<object>
     reads this, list
@@ -21,8 +10,19 @@ class DoublyLinkedListWithLast {
     list.Repr()
   }
 
+  predicate Valid()
+    reads this, list, Repr()
+  {
+    && list.Valid()
+      && (if last == null then
+      list.head == null
+      else
+        last in list.Repr() && last.next == null
+        )
+  }
+
   function Model(): seq<A>
-    reads this, list, list.spine
+    reads this, list, Repr()
     requires Valid()
   {
     list.Model()
@@ -31,16 +31,16 @@ class DoublyLinkedListWithLast {
   constructor()
     ensures Valid()
     ensures Model() == []
+    ensures fresh(Repr())
     ensures fresh(list)
     ensures last == null
-    ensures fresh(Repr())
   {
-    list := new DoublyLinkedList();
+    list := new List();
     last := null;
   }
 
-  function method Front(): int
-    reads this, list, list.Repr()
+  function method Front(): A
+    reads this, list, Repr()
     requires Valid()
     requires Model() != []
     ensures Valid()
@@ -49,21 +49,9 @@ class DoublyLinkedListWithLast {
     list.head.data
   }
 
-  function method Back(): int
-    reads this, list, list.Repr()
-    requires Valid()
-    requires Model() != []
-    ensures Valid()
-    ensures Back() == Model()[|Model()|-1]
-  {
-    list.LastHasLastIndex(last);
-    list.ModelRelationWithSpine();
-    last.data
-  }
-
   // O(1)
   method PushFront(x: A)
-    modifies this, list, Repr()
+    modifies this, list
     requires Valid()
     ensures Valid()
     ensures Model() == [x] + old(Model())
@@ -72,12 +60,7 @@ class DoublyLinkedListWithLast {
     ensures list == old(list)
   {
     var ohead := list.head;
-    { // GHOST
-      if ohead != null {
-        list.LastHasLastIndex(last);
-      }
-    }
-    list.PushFront(x);
+    list.Push(x);
     if ohead == null {
       last := list.head;
     }
@@ -85,36 +68,23 @@ class DoublyLinkedListWithLast {
 
   // O(1)
   method PopFront() returns (x: A)
-    modifies this, list, Repr()
+    modifies this, list
     requires Valid()
     requires Model() != []
     ensures Valid()
     ensures [x] + Model() == old(Model())
     ensures Repr() < old(Repr())
     ensures list == old(list)
-    ensures [old(list.head)] + list.spine == old(list.spine);
   {
-    { // GHOST
-      if list.head != null {
-        list.LastHasLastIndex(last);
-      }
-    }
     if list.head == last {
       last := null;
     }
-    { // GHOST
-      if list.head.next != null {
-        assert list.head == list.spine[0];
-        assert list.head.next == list.spine[1];
-        assert list.head.next in Repr();
-      }
-    }
-    x := list.PopFront();
+    x := list.Pop();
   }
 
   // O(1)
   method PushBack(x: A)
-    modifies this, list, Repr()
+    modifies this, last, list
     requires Valid()
     ensures Valid()
     ensures Model() == old(Model()) + [x]
@@ -124,7 +94,7 @@ class DoublyLinkedListWithLast {
   {
     if last == null {
       assert Model() == [];
-      list.PushFront(x);
+      list.Push(x);
       last := list.head;
     } else {
       { // GHOST
@@ -138,7 +108,7 @@ class DoublyLinkedListWithLast {
     }
   }
 
-  // O(1)
+  // O(n)
   method PopBack() returns (x: A)
     modifies this, list, list.Repr()
     requires Valid()
@@ -147,7 +117,6 @@ class DoublyLinkedListWithLast {
     ensures Model() + [x] == old(Model())
     ensures Repr() < old(Repr())
     ensures list == old(list)
-    ensures list.spine + [old(last)] == old(list.spine)
   {
     if list.head == last {
       assert list.head.next == null;
@@ -166,18 +135,15 @@ class DoublyLinkedListWithLast {
       assert Model() + [x] == old(Model());
       assert Repr() < old(Repr());
     } else {
-      x := last.data;
-      var prev := last.prev;
-      { // GHOST
-        list.ModelRelationWithSpine();
-        list.LastHasLastIndex(last);
-        assert last == list.spine[|list.spine|-1];
-        assert last.prev == list.spine[|list.spine|-2];
-        assert prev in Repr();
-        assert last in Repr();
-      }
+      /*GHOST*/ list.ModelRelationWithSpine();
+      var prev := list.FindPrev(last);
+      assert prev in Repr();
+      assert last in Repr();
+      /*GHOST*/ list.PrevHasPrevIndex(prev, last);
       list.RemoveNext(prev);
+      x := last.data;
       last := prev;
+      /*GHOST*/ list.LastHasLastIndex(last);
     }
   }
 }
